PREFIX : <http://pid.suncorp.com.au/def/brand/suncorp-anzsic/>
PREFIX anzsic: <http://linked.data.gov.au/def/anzsic-2006>
PREFIX cs: <http://pid.suncorp.com.au/def/suncorp-anzsic>
PREFIX dcterms: <http://purl.org/dc/terms/>
PREFIX rdfs: <http://www.w3.org/2000/01/rdf-schema#>
PREFIX schema: <https://schema.org/>
PREFIX skos: <http://www.w3.org/2004/02/skos/core#>
PREFIX xsd: <http://www.w3.org/2001/XMLSchema#>

:A0110
    a skos:Concept ;
    rdfs:isDefinedBy anzsic: ;
    skos:broader :A0100 ;
    skos:definition "An individual business entity whose predominant economic activity is Nursery and Floriculture Production."@en ;
    skos:inScheme cs: ;
    skos:notation "A0110" ;
    skos:prefLabel "Nursery and Floriculture Production"@en ;
    schema:temporalCoverage
        [
            schema:startTime "2026-02-10"^^xsd:date ;
        ] ;
.

:A0120
    a skos:Concept ;
    rdfs:isDefinedBy anzsic: ;
    skos:broader :A0100 ;
    skos:definition "An individual business entity whose predominant economic activity is Mushroom and Vegetable Growing."@en ;
    skos:inScheme cs: ;
    skos:notation "A0120" ;
    skos:prefLabel "Mushroom and Vegetable Growing"@en ;
    schema:temporalCoverage
        [
            schema:startTime "2026-02-10"^^xsd:date ;
        ] ;
.

:A0130
    a skos:Concept ;
    rdfs:isDefinedBy anzsic: ;
    skos:broader :A0100 ;
    skos:definition "An individual business entity whose predominant economic activity is Fruit and Tree Nut Growing."@en ;
    skos:inScheme cs: ;
    skos:notation "A0130" ;
    skos:prefLabel "Fruit and Tree Nut Growing"@en ;
    schema:temporalCoverage
        [
            schema:startTime "2026-02-10"^^xsd:date ;
        ] ;
.

:A0140
    a skos:Concept ;
    rdfs:isDefinedBy anzsic: ;
    skos:broader :A0100 ;
    skos:definition "An individual business entity whose predominant economic activity is Sheep, Beef Cattle and Grain Farming."@en ;
    skos:inScheme cs: ;
    skos:notation "A0140" ;
    skos:prefLabel "Sheep, Beef Cattle and Grain Farming"@en ;
    schema:temporalCoverage
        [
            schema:startTime "2026-02-10"^^xsd:date ;
        ] ;
.

:A0150
    a skos:Concept ;
    rdfs:isDefinedBy anzsic: ;
    skos:broader :A0100 ;
    skos:definition "An individual business entity whose predominant economic activity is Other Crop Growing."@en ;
    skos:inScheme cs: ;
    skos:notation "A0150" ;
    skos:prefLabel "Other Crop Growing"@en ;
    schema:temporalCoverage
        [
            schema:startTime "2026-02-10"^^xsd:date ;
        ] ;
.

:A0160
    a skos:Concept ;
    rdfs:isDefinedBy anzsic: ;
    skos:broader :A0100 ;
    skos:definition "An individual business entity whose predominant economic activity is Dairy Cattle Farming."@en ;
    skos:inScheme cs: ;
    skos:notation "A0160" ;
    skos:prefLabel "Dairy Cattle Farming"@en ;
    schema:temporalCoverage
        [
            schema:startTime "2026-02-10"^^xsd:date ;
        ] ;
.

:A0170
    a skos:Concept ;
    rdfs:isDefinedBy anzsic: ;
    skos:broader :A0100 ;
    skos:definition "An individual business entity whose predominant economic activity is Poultry Farming."@en ;
    skos:inScheme cs: ;
    skos:notation "A0170" ;
    skos:prefLabel "Poultry Farming"@en ;
    schema:temporalCoverage
        [
            schema:startTime "2026-02-10"^^xsd:date ;
        ] ;
.

:A0180
    a skos:Concept ;
    rdfs:isDefinedBy anzsic: ;
    skos:broader :A0100 ;
    skos:definition "An individual business entity whose predominant economic activity is Deer Farming."@en ;
    skos:inScheme cs: ;
    skos:notation "A0180" ;
    skos:prefLabel "Deer Farming"@en ;
    schema:temporalCoverage
        [
            schema:startTime "2026-02-10"^^xsd:date ;
        ] ;
.

:A0190
    a skos:Concept ;
    rdfs:isDefinedBy anzsic: ;
    skos:broader :A0100 ;
    skos:definition "An individual business entity whose predominant economic activity is Other Livestock Farming."@en ;
    skos:inScheme cs: ;
    skos:notation "A0190" ;
    skos:prefLabel "Other Livestock Farming"@en ;
    schema:temporalCoverage
        [
            schema:startTime "2026-02-10"^^xsd:date ;
        ] ;
.

:A0200
    a skos:Concept ;
    rdfs:isDefinedBy anzsic: ;
    skos:broader :A0000 ;
    skos:definition "An individual business entity whose predominant economic activity is Aquaculture."@en ;
    skos:inScheme cs: ;
    skos:notation "A0200" ;
    skos:prefLabel "Aquaculture"@en ;
    schema:temporalCoverage
        [
            schema:startTime "2026-02-10"^^xsd:date ;
        ] ;
.

:A0300
    a skos:Concept ;
    rdfs:isDefinedBy anzsic: ;
    skos:broader :A0000 ;
    skos:definition "An individual business entity whose predominant economic activity is Forestry and Logging."@en ;
    skos:inScheme cs: ;
    skos:notation "A0300" ;
    skos:prefLabel "Forestry and Logging"@en ;
    schema:temporalCoverage
        [
            schema:startTime "2026-02-10"^^xsd:date ;
        ] ;
.

:A0410
    a skos:Concept ;
    rdfs:isDefinedBy anzsic: ;
    skos:broader :A0400 ;
    skos:definition "An individual business entity whose predominant economic activity is Fishing."@en ;
    skos:inScheme cs: ;
    skos:notation "A0410" ;
    skos:prefLabel "Fishing"@en ;
    schema:temporalCoverage
        [
            schema:startTime "2026-02-10"^^xsd:date ;
        ] ;
.

:A0420
    a skos:Concept ;
    rdfs:isDefinedBy anzsic: ;
    skos:broader :A0400 ;
    skos:definition "An individual business entity whose predominant economic activity is Hunting and Trapping."@en ;
    skos:inScheme cs: ;
    skos:notation "A0420" ;
    skos:prefLabel "Hunting and Trapping"@en ;
    schema:temporalCoverage
        [
            schema:startTime "2026-02-10"^^xsd:date ;
        ] ;
.

:A0510
    a skos:Concept ;
    rdfs:isDefinedBy anzsic: ;
    skos:broader :A0500 ;
    skos:definition "An individual business entity whose predominant economic activity is Forestry Support Services."@en ;
    skos:inScheme cs: ;
    skos:notation "A0510" ;
    skos:prefLabel "Forestry Support Services"@en ;
    schema:temporalCoverage
        [
            schema:startTime "2026-02-10"^^xsd:date ;
        ] ;
.

:A0520
    a skos:Concept ;
    rdfs:isDefinedBy anzsic: ;
    skos:broader :A0500 ;
    skos:definition "An individual business entity whose predominant economic activity is Agriculture and Fishing Support Services."@en ;
    skos:inScheme cs: ;
    skos:notation "A0520" ;
    skos:prefLabel "Agriculture and Fishing Support Services"@en ;
    schema:temporalCoverage
        [
            schema:startTime "2026-02-10"^^xsd:date ;
        ] ;
.

:B0600
    a skos:Concept ;
    rdfs:isDefinedBy anzsic: ;
    skos:altLabel "Coal Mine"@en ;
    skos:broader :B0000 ;
    skos:definition "An individual business entity whose predominant economic activity is Coal Mining."@en ;
    skos:inScheme cs: ;
    skos:notation "B0600" ;
    skos:prefLabel "Coal Mining"@en ;
    schema:temporalCoverage
        [
            schema:startTime "2026-02-10"^^xsd:date ;
        ] ;
.

:B0700
    a skos:Concept ;
    rdfs:isDefinedBy anzsic: ;
    skos:broader :B0000 ;
    skos:definition "An individual business entity whose predominant economic activity is Oil and Gas Extraction."@en ;
    skos:inScheme cs: ;
    skos:notation "B0700" ;
    skos:prefLabel "Oil and Gas Extraction"@en ;
    schema:temporalCoverage
        [
            schema:startTime "2026-02-10"^^xsd:date ;
        ] ;
.

:B0800
    a skos:Concept ;
    rdfs:isDefinedBy anzsic: ;
    skos:broader :B0000 ;
    skos:definition "An individual business entity whose predominant economic activity is Metal Ore Mining."@en ;
    skos:inScheme cs: ;
    skos:notation "B0800" ;
    skos:prefLabel "Metal Ore Mining"@en ;
    schema:temporalCoverage
        [
            schema:startTime "2026-02-10"^^xsd:date ;
        ] ;
.

:B0910
    a skos:Concept ;
    rdfs:isDefinedBy anzsic: ;
    skos:broader :B0900 ;
    skos:definition "An individual business entity whose predominant economic activity is Construction Material Mining."@en ;
    skos:inScheme cs: ;
    skos:notation "B0910" ;
    skos:prefLabel "Construction Material Mining"@en ;
    schema:temporalCoverage
        [
            schema:startTime "2026-02-10"^^xsd:date ;
        ] ;
.

:B0990
    a skos:Concept ;
    rdfs:isDefinedBy anzsic: ;
    skos:broader :B0900 ;
    skos:definition "An individual business entity whose predominant economic activity is Other Non-Metallic Mineral Mining and Quarrying."@en ;
    skos:inScheme cs: ;
    skos:notation "B0990" ;
    skos:prefLabel "Other Non-Metallic Mineral Mining and Quarrying"@en ;
    schema:temporalCoverage
        [
            schema:startTime "2026-02-10"^^xsd:date ;
        ] ;
.

:B1010
    a skos:Concept ;
    rdfs:isDefinedBy anzsic: ;
    skos:broader :B1000 ;
    skos:definition "An individual business entity whose predominant economic activity is Exploration."@en ;
    skos:inScheme cs: ;
    skos:notation "B1010" ;
    skos:prefLabel "Exploration"@en ;
    schema:temporalCoverage
        [
            schema:startTime "2026-02-10"^^xsd:date ;
        ] ;
.

:B1090
    a skos:Concept ;
    rdfs:isDefinedBy anzsic: ;
    skos:broader :B1000 ;
    skos:definition "An individual business entity whose predominant economic activity is Other Mining Support Services."@en ;
    skos:inScheme cs: ;
    skos:notation "B1090" ;
    skos:prefLabel "Other Mining Support Services"@en ;
    schema:temporalCoverage
        [
            schema:startTime "2026-02-10"^^xsd:date ;
        ] ;
.

:C1110
    a skos:Concept ;
    rdfs:isDefinedBy anzsic: ;
    skos:broader :C1100 ;
    skos:definition "An individual business entity whose predominant economic activity is Meat and Meat Product Manufacturing."@en ;
    skos:inScheme cs: ;
    skos:notation "C1110" ;
    skos:prefLabel "Meat and Meat Product Manufacturing"@en ;
    schema:temporalCoverage
        [
            schema:startTime "2026-02-10"^^xsd:date ;
        ] ;
.

:C1120
    a skos:Concept ;
    rdfs:isDefinedBy anzsic: ;
    skos:broader :C1100 ;
    skos:definition "An individual business entity whose predominant economic activity is Seafood Processing."@en ;
    skos:inScheme cs: ;
    skos:notation "C1120" ;
    skos:prefLabel "Seafood Processing"@en ;
    schema:temporalCoverage
        [
            schema:startTime "2026-02-10"^^xsd:date ;
        ] ;
.

:C1130
    a skos:Concept ;
    rdfs:isDefinedBy anzsic: ;
    skos:broader :C1100 ;
    skos:definition "An individual business entity whose predominant economic activity is Dairy Product Manufacturing."@en ;
    skos:inScheme cs: ;
    skos:notation "C1130" ;
    skos:prefLabel "Dairy Product Manufacturing"@en ;
    schema:temporalCoverage
        [
            schema:startTime "2026-02-10"^^xsd:date ;
        ] ;
.

:C1140
    a skos:Concept ;
    rdfs:isDefinedBy anzsic: ;
    skos:broader :C1100 ;
    skos:definition "An individual business entity whose predominant economic activity is Fruit and Vegetable Processing."@en ;
    skos:inScheme cs: ;
    skos:notation "C1140" ;
    skos:prefLabel "Fruit and Vegetable Processing"@en ;
    schema:temporalCoverage
        [
            schema:startTime "2026-02-10"^^xsd:date ;
        ] ;
.

:C1150
    a skos:Concept ;
    rdfs:isDefinedBy anzsic: ;
    skos:broader :C1100 ;
    skos:definition "An individual business entity whose predominant economic activity is Oil and Fat Manufacturing."@en ;
    skos:inScheme cs: ;
    skos:notation "C1150" ;
    skos:prefLabel "Oil and Fat Manufacturing"@en ;
    schema:temporalCoverage
        [
            schema:startTime "2026-02-10"^^xsd:date ;
        ] ;
.

:C1160
    a skos:Concept ;
    rdfs:isDefinedBy anzsic: ;
    skos:broader :C1100 ;
    skos:definition "An individual business entity whose predominant economic activity is Grain Mill and Cereal Product Manufacturing."@en ;
    skos:inScheme cs: ;
    skos:notation "C1160" ;
    skos:prefLabel "Grain Mill and Cereal Product Manufacturing"@en ;
    schema:temporalCoverage
        [
            schema:startTime "2026-02-10"^^xsd:date ;
        ] ;
.

:C1170
    a skos:Concept ;
    rdfs:isDefinedBy anzsic: ;
    skos:broader :C1100 ;
    skos:definition "An individual business entity whose predominant economic activity is Bakery Product Manufacturing."@en ;
    skos:inScheme cs: ;
    skos:notation "C1170" ;
    skos:prefLabel "Bakery Product Manufacturing"@en ;
    schema:temporalCoverage
        [
            schema:startTime "2026-02-10"^^xsd:date ;
        ] ;
.

:C1180
    a skos:Concept ;
    rdfs:isDefinedBy anzsic: ;
    skos:broader :C1100 ;
    skos:definition "An individual business entity whose predominant economic activity is Sugar and Confectionery Manufacturing."@en ;
    skos:inScheme cs: ;
    skos:notation "C1180" ;
    skos:prefLabel "Sugar and Confectionery Manufacturing"@en ;
    schema:temporalCoverage
        [
            schema:startTime "2026-02-10"^^xsd:date ;
        ] ;
.

:C1190
    a skos:Concept ;
    rdfs:isDefinedBy anzsic: ;
    skos:broader :C1100 ;
    skos:definition "An individual business entity whose predominant economic activity is Other Food Product Manufacturing."@en ;
    skos:inScheme cs: ;
    skos:notation "C1190" ;
    skos:prefLabel "Other Food Product Manufacturing"@en ;
    schema:temporalCoverage
        [
            schema:startTime "2026-02-10"^^xsd:date ;
        ] ;
.

:C1210
    a skos:Concept ;
    rdfs:isDefinedBy anzsic: ;
    skos:broader :C1200 ;
    skos:definition "An individual business entity whose predominant economic activity is Beverage Manufacturing."@en ;
    skos:inScheme cs: ;
    skos:notation "C1210" ;
    skos:prefLabel "Beverage Manufacturing"@en ;
    schema:temporalCoverage
        [
            schema:startTime "2026-02-10"^^xsd:date ;
        ] ;
.

:C1220
    a skos:Concept ;
    rdfs:isDefinedBy anzsic: ;
    skos:broader :C1200 ;
    skos:definition "An individual business entity whose predominant economic activity is Cigarette and Tobacco Product Manufacturing."@en ;
    skos:inScheme cs: ;
    skos:notation "C1220" ;
    skos:prefLabel "Cigarette and Tobacco Product Manufacturing"@en ;
    schema:temporalCoverage
        [
            schema:startTime "2026-02-10"^^xsd:date ;
        ] ;
.

:C1310
    a skos:Concept ;
    rdfs:isDefinedBy anzsic: ;
    skos:broader :C1300 ;
    skos:definition "An individual business entity whose predominant economic activity is Textile Manufacturing."@en ;
    skos:inScheme cs: ;
    skos:notation "C1310" ;
    skos:prefLabel "Textile Manufacturing"@en ;
    schema:temporalCoverage
        [
            schema:startTime "2026-02-10"^^xsd:date ;
        ] ;
.

:C1320
    a skos:Concept ;
    rdfs:isDefinedBy anzsic: ;
    skos:broader :C1300 ;
    skos:definition "An individual business entity whose predominant economic activity is Leather Tanning, Fur Dressing and Leather Product Manufacturing."@en ;
    skos:inScheme cs: ;
    skos:notation "C1320" ;
    skos:prefLabel "Leather Tanning, Fur Dressing and Leather Product Manufacturing"@en ;
    schema:temporalCoverage
        [
            schema:startTime "2026-02-10"^^xsd:date ;
        ] ;
.

:C1330
    a skos:Concept ;
    rdfs:isDefinedBy anzsic: ;
    skos:broader :C1300 ;
    skos:definition "An individual business entity whose predominant economic activity is Textile Product Manufacturing."@en ;
    skos:inScheme cs: ;
    skos:notation "C1330" ;
    skos:prefLabel "Textile Product Manufacturing"@en ;
    schema:temporalCoverage
        [
            schema:startTime "2026-02-10"^^xsd:date ;
        ] ;
.

:C1340
    a skos:Concept ;
    rdfs:isDefinedBy anzsic: ;
    skos:broader :C1300 ;
    skos:definition "An individual business entity whose predominant economic activity is Knitted Product Manufacturing."@en ;
    skos:inScheme cs: ;
    skos:notation "C1340" ;
    skos:prefLabel "Knitted Product Manufacturing"@en ;
    schema:temporalCoverage
        [
            schema:startTime "2026-02-10"^^xsd:date ;
        ] ;
.

:C1350
    a skos:Concept ;
    rdfs:isDefinedBy anzsic: ;
    skos:broader :C1300 ;
    skos:definition "An individual business entity whose predominant economic activity is Clothing and Footwear Manufacturing."@en ;
    skos:inScheme cs: ;
    skos:notation "C1350" ;
    skos:prefLabel "Clothing and Footwear Manufacturing"@en ;
    schema:temporalCoverage
        [
            schema:startTime "2026-02-10"^^xsd:date ;
        ] ;
.

:C1410
    a skos:Concept ;
    rdfs:isDefinedBy anzsic: ;
    skos:broader :C1400 ;
    skos:definition "An individual business entity whose predominant economic activity is Log Sawmilling and Timber Dressing."@en ;
    skos:inScheme cs: ;
    skos:notation "C1410" ;
    skos:prefLabel "Log Sawmilling and Timber Dressing"@en ;
    schema:temporalCoverage
        [
            schema:startTime "2026-02-10"^^xsd:date ;
        ] ;
.

:C1490
    a skos:Concept ;
    rdfs:isDefinedBy anzsic: ;
    skos:broader :C1400 ;
    skos:definition "An individual business entity whose predominant economic activity is Other Wood Product Manufacturing."@en ;
    skos:inScheme cs: ;
    skos:notation "C1490" ;
    skos:prefLabel "Other Wood Product Manufacturing"@en ;
    schema:temporalCoverage
        [
            schema:startTime "2026-02-10"^^xsd:date ;
        ] ;
.

:C1510x
    a skos:Concept ;
    rdfs:isDefinedBy cs: ;
    skos:broader :C1510 ;
    skos:definition "An individual business entity whose predominant economic activity is toilet paper Manufacturing."@en ;
    skos:inScheme cs: ;
    skos:notation "C1510x" ;
    skos:prefLabel "Toilet paper Manufacturing"@en ;
    schema:creator <https://orcid.org/0000-0002-8742-7730> ;
    schema:temporalCoverage
        [
            schema:startTime "2026-02-11"^^xsd:date ;
        ] ;
.

:C1520
    a skos:Concept ;
    rdfs:isDefinedBy anzsic: ;
    skos:broader :C1500 ;
    skos:definition "An individual business entity whose predominant economic activity is Converted Paper Product Manufacturing."@en ;
    skos:inScheme cs: ;
    skos:notation "C1520" ;
    skos:prefLabel "Converted Paper Product Manufacturing"@en ;
    schema:temporalCoverage
        [
            schema:startTime "2026-02-10"^^xsd:date ;
        ] ;
.

:C1610
    a skos:Concept ;
    rdfs:isDefinedBy anzsic: ;
    skos:broader :C1600 ;
    skos:definition "An individual business entity whose predominant economic activity is Printing and Printing Support Services."@en ;
    skos:inScheme cs: ;
    skos:notation "C1610" ;
    skos:prefLabel "Printing and Printing Support Services"@en ;
    schema:temporalCoverage
        [
            schema:startTime "2026-02-10"^^xsd:date ;
        ] ;
.

:C1620
    a skos:Concept ;
    rdfs:isDefinedBy anzsic: ;
    skos:broader :C1600 ;
    skos:definition "An individual business entity whose predominant economic activity is Reproduction of Recorded Media."@en ;
    skos:inScheme cs: ;
    skos:notation "C1620" ;
    skos:prefLabel "Reproduction of Recorded Media"@en ;
    schema:temporalCoverage
        [
            schema:startTime "2026-02-10"^^xsd:date ;
        ] ;
.

:C1700
    a skos:Concept ;
    rdfs:isDefinedBy anzsic: ;
    skos:broader :C0000 ;
    skos:definition "An individual business entity whose predominant economic activity is Petroleum and Coal Product Manufacturing."@en ;
    skos:inScheme cs: ;
    skos:notation "C1700" ;
    skos:prefLabel "Petroleum and Coal Product Manufacturing"@en ;
    schema:temporalCoverage
        [
            schema:startTime "2026-02-10"^^xsd:date ;
        ] ;
.

:C1810
    a skos:Concept ;
    rdfs:isDefinedBy anzsic: ;
    skos:broader :C1800 ;
    skos:definition "An individual business entity whose predominant economic activity is Basic Chemical Manufacturing."@en ;
    skos:inScheme cs: ;
    skos:notation "C1810" ;
    skos:prefLabel "Basic Chemical Manufacturing"@en ;
    schema:temporalCoverage
        [
            schema:startTime "2026-02-10"^^xsd:date ;
        ] ;
.

:C1820
    a skos:Concept ;
    rdfs:isDefinedBy anzsic: ;
    skos:broader :C1800 ;
    skos:definition "An individual business entity whose predominant economic activity is Basic Polymer Manufacturing."@en ;
    skos:inScheme cs: ;
    skos:notation "C1820" ;
    skos:prefLabel "Basic Polymer Manufacturing"@en ;
    schema:temporalCoverage
        [
            schema:startTime "2026-02-10"^^xsd:date ;
        ] ;
.

:C1830
    a skos:Concept ;
    rdfs:isDefinedBy anzsic: ;
    skos:broader :C1800 ;
    skos:definition "An individual business entity whose predominant economic activity is Fertiliser and Pesticide Manufacturing."@en ;
    skos:inScheme cs: ;
    skos:notation "C1830" ;
    skos:prefLabel "Fertiliser and Pesticide Manufacturing"@en ;
    schema:temporalCoverage
        [
            schema:startTime "2026-02-10"^^xsd:date ;
        ] ;
.

:C1840
    a skos:Concept ;
    rdfs:isDefinedBy anzsic: ;
    skos:broader :C1800 ;
    skos:definition "An individual business entity whose predominant economic activity is Pharmaceutical and Medicinal Product Manufacturing."@en ;
    skos:inScheme cs: ;
    skos:notation "C1840" ;
    skos:prefLabel "Pharmaceutical and Medicinal Product Manufacturing"@en ;
    schema:temporalCoverage
        [
            schema:startTime "2026-02-10"^^xsd:date ;
        ] ;
.

:C1850
    a skos:Concept ;
    rdfs:isDefinedBy anzsic: ;
    skos:broader :C1800 ;
    skos:definition "An individual business entity whose predominant economic activity is Cleaning Compound and Toiletry Preparation Manufacturing."@en ;
    skos:inScheme cs: ;
    skos:notation "C1850" ;
    skos:prefLabel "Cleaning Compound and Toiletry Preparation Manufacturing"@en ;
    schema:temporalCoverage
        [
            schema:startTime "2026-02-10"^^xsd:date ;
        ] ;
.

:C1890
    a skos:Concept ;
    rdfs:isDefinedBy anzsic: ;
    skos:broader :C1800 ;
    skos:definition "An individual business entity whose predominant economic activity is Other Basic Chemical Product Manufacturing."@en ;
    skos:inScheme cs: ;
    skos:notation "C1890" ;
    skos:prefLabel "Other Basic Chemical Product Manufacturing"@en ;
    schema:temporalCoverage
        [
            schema:startTime "2026-02-10"^^xsd:date ;
        ] ;
.

:C1910
    a skos:Concept ;
    rdfs:isDefinedBy anzsic: ;
    skos:broader :C1900 ;
    skos:definition "An individual business entity whose predominant economic activity is Polymer Product Manufacturing."@en ;
    skos:inScheme cs: ;
    skos:notation "C1910" ;
    skos:prefLabel "Polymer Product Manufacturing"@en ;
    schema:temporalCoverage
        [
            schema:startTime "2026-02-10"^^xsd:date ;
        ] ;
.

:C1920
    a skos:Concept ;
    rdfs:isDefinedBy anzsic: ;
    skos:broader :C1900 ;
    skos:definition "An individual business entity whose predominant economic activity is Natural Rubber Product Manufacturing."@en ;
    skos:inScheme cs: ;
    skos:notation "C1920" ;
    skos:prefLabel "Natural Rubber Product Manufacturing"@en ;
    schema:temporalCoverage
        [
            schema:startTime "2026-02-10"^^xsd:date ;
        ] ;
.

:C2010
    a skos:Concept ;
    rdfs:isDefinedBy anzsic: ;
    skos:broader :C2000 ;
    skos:definition "An individual business entity whose predominant economic activity is Glass and Glass Product Manufacturing."@en ;
    skos:inScheme cs: ;
    skos:notation "C2010" ;
    skos:prefLabel "Glass and Glass Product Manufacturing"@en ;
    schema:temporalCoverage
        [
            schema:startTime "2026-02-10"^^xsd:date ;
        ] ;
.

:C2020
    a skos:Concept ;
    rdfs:isDefinedBy anzsic: ;
    skos:broader :C2000 ;
    skos:definition "An individual business entity whose predominant economic activity is Ceramic Product Manufacturing."@en ;
    skos:inScheme cs: ;
    skos:notation "C2020" ;
    skos:prefLabel "Ceramic Product Manufacturing"@en ;
    schema:temporalCoverage
        [
            schema:startTime "2026-02-10"^^xsd:date ;
        ] ;
.

:C2030
    a skos:Concept ;
    rdfs:isDefinedBy anzsic: ;
    skos:broader :C2000 ;
    skos:definition "An individual business entity whose predominant economic activity is Cement, Lime, Plaster and Concrete Product Manufacturing."@en ;
    skos:inScheme cs: ;
    skos:notation "C2030" ;
    skos:prefLabel "Cement, Lime, Plaster and Concrete Product Manufacturing"@en ;
    schema:temporalCoverage
        [
            schema:startTime "2026-02-10"^^xsd:date ;
        ] ;
.

:C2090
    a skos:Concept ;
    rdfs:isDefinedBy anzsic: ;
    skos:broader :C2000 ;
    skos:definition "An individual business entity whose predominant economic activity is Other Non-Metallic Mineral Product Manufacturing."@en ;
    skos:inScheme cs: ;
    skos:notation "C2090" ;
    skos:prefLabel "Other Non-Metallic Mineral Product Manufacturing"@en ;
    schema:temporalCoverage
        [
            schema:startTime "2026-02-10"^^xsd:date ;
        ] ;
.

:C2110
    a skos:Concept ;
    rdfs:isDefinedBy anzsic: ;
    skos:broader :C2100 ;
    skos:definition "An individual business entity whose predominant economic activity is Basic Ferrous Metal Manufacturing."@en ;
    skos:inScheme cs: ;
    skos:notation "C2110" ;
    skos:prefLabel "Basic Ferrous Metal Manufacturing"@en ;
    schema:temporalCoverage
        [
            schema:startTime "2026-02-10"^^xsd:date ;
        ] ;
.

:C2120
    a skos:Concept ;
    rdfs:isDefinedBy anzsic: ;
    skos:broader :C2100 ;
    skos:definition "An individual business entity whose predominant economic activity is Basic Ferrous Metal Product Manufacturing."@en ;
    skos:inScheme cs: ;
    skos:notation "C2120" ;
    skos:prefLabel "Basic Ferrous Metal Product Manufacturing"@en ;
    schema:temporalCoverage
        [
            schema:startTime "2026-02-10"^^xsd:date ;
        ] ;
.

:C2130
    a skos:Concept ;
    rdfs:isDefinedBy anzsic: ;
    skos:broader :C2100 ;
    skos:definition "An individual business entity whose predominant economic activity is Basic Non-Ferrous Metal Manufacturing."@en ;
    skos:inScheme cs: ;
    skos:notation "C2130" ;
    skos:prefLabel "Basic Non-Ferrous Metal Manufacturing"@en ;
    schema:temporalCoverage
        [
            schema:startTime "2026-02-10"^^xsd:date ;
        ] ;
.

:C2140
    a skos:Concept ;
    rdfs:isDefinedBy anzsic: ;
    skos:broader :C2100 ;
    skos:definition "An individual business entity whose predominant economic activity is Basic Non-Ferrous Metal Product Manufacturing."@en ;
    skos:inScheme cs: ;
    skos:notation "C2140" ;
    skos:prefLabel "Basic Non-Ferrous Metal Product Manufacturing"@en ;
    schema:temporalCoverage
        [
            schema:startTime "2026-02-10"^^xsd:date ;
        ] ;
.

:C2210
    a skos:Concept ;
    rdfs:isDefinedBy anzsic: ;
    skos:broader :C2200 ;
    skos:definition "An individual business entity whose predominant economic activity is Iron and Steel Forging."@en ;
    skos:inScheme cs: ;
    skos:notation "C2210" ;
    skos:prefLabel "Iron and Steel Forging"@en ;
    schema:temporalCoverage
        [
            schema:startTime "2026-02-10"^^xsd:date ;
        ] ;
.

:C2220
    a skos:Concept ;
    rdfs:isDefinedBy anzsic: ;
    skos:broader :C2200 ;
    skos:definition "An individual business entity whose predominant economic activity is Structural Metal Product Manufacturing."@en ;
    skos:inScheme cs: ;
    skos:notation "C2220" ;
    skos:prefLabel "Structural Metal Product Manufacturing"@en ;
    schema:temporalCoverage
        [
            schema:startTime "2026-02-10"^^xsd:date ;
        ] ;
.

:C2230
    a skos:Concept ;
    rdfs:isDefinedBy anzsic: ;
    skos:broader :C2200 ;
    skos:definition "An individual business entity whose predominant economic activity is Metal Container Manufacturing."@en ;
    skos:inScheme cs: ;
    skos:notation "C2230" ;
    skos:prefLabel "Metal Container Manufacturing"@en ;
    schema:temporalCoverage
        [
            schema:startTime "2026-02-10"^^xsd:date ;
        ] ;
.

:C2240
    a skos:Concept ;
    rdfs:isDefinedBy anzsic: ;
    skos:broader :C2200 ;
    skos:definition "An individual business entity whose predominant economic activity is Sheet Metal Product Manufacturing (except Metal Structural and Container Products)."@en ;
    skos:inScheme cs: ;
    skos:notation "C2240" ;
    skos:prefLabel "Sheet Metal Product Manufacturing (except Metal Structural and Container Products)"@en ;
    schema:temporalCoverage
        [
            schema:startTime "2026-02-10"^^xsd:date ;
        ] ;
.

:C2290
    a skos:Concept ;
    rdfs:isDefinedBy anzsic: ;
    skos:broader :C2200 ;
    skos:definition "An individual business entity whose predominant economic activity is Other Fabricated Metal Product Manufacturing."@en ;
    skos:inScheme cs: ;
    skos:notation "C2290" ;
    skos:prefLabel "Other Fabricated Metal Product Manufacturing"@en ;
    schema:temporalCoverage
        [
            schema:startTime "2026-02-10"^^xsd:date ;
        ] ;
.

:C2310
    a skos:Concept ;
    rdfs:isDefinedBy anzsic: ;
    skos:broader :C2300 ;
    skos:definition "An individual business entity whose predominant economic activity is Motor Vehicle and Motor Vehicle Part Manufacturing."@en ;
    skos:inScheme cs: ;
    skos:notation "C2310" ;
    skos:prefLabel "Motor Vehicle and Motor Vehicle Part Manufacturing"@en ;
    schema:temporalCoverage
        [
            schema:startTime "2026-02-10"^^xsd:date ;
        ] ;
.

:C2390
    a skos:Concept ;
    rdfs:isDefinedBy anzsic: ;
    skos:broader :C2300 ;
    skos:definition "An individual business entity whose predominant economic activity is Other Transport Equipment Manufacturing."@en ;
    skos:inScheme cs: ;
    skos:notation "C2390" ;
    skos:prefLabel "Other Transport Equipment Manufacturing"@en ;
    schema:temporalCoverage
        [
            schema:startTime "2026-02-10"^^xsd:date ;
        ] ;
.

:C2410
    a skos:Concept ;
    rdfs:isDefinedBy anzsic: ;
    skos:broader :C2400 ;
    skos:definition "An individual business entity whose predominant economic activity is Professional and Scientific Equipment Manufacturing."@en ;
    skos:inScheme cs: ;
    skos:notation "C2410" ;
    skos:prefLabel "Professional and Scientific Equipment Manufacturing"@en ;
    schema:temporalCoverage
        [
            schema:startTime "2026-02-10"^^xsd:date ;
        ] ;
.

:C2420
    a skos:Concept ;
    rdfs:isDefinedBy anzsic: ;
    skos:broader :C2400 ;
    skos:definition "An individual business entity whose predominant economic activity is Computer and Electronic Equipment Manufacturing."@en ;
    skos:inScheme cs: ;
    skos:notation "C2420" ;
    skos:prefLabel "Computer and Electronic Equipment Manufacturing"@en ;
    schema:temporalCoverage
        [
            schema:startTime "2026-02-10"^^xsd:date ;
        ] ;
.

:C2430
    a skos:Concept ;
    rdfs:isDefinedBy anzsic: ;
    skos:broader :C2400 ;
    skos:definition "An individual business entity whose predominant economic activity is Electrical Equipment Manufacturing."@en ;
    skos:inScheme cs: ;
    skos:notation "C2430" ;
    skos:prefLabel "Electrical Equipment Manufacturing"@en ;
    schema:temporalCoverage
        [
            schema:startTime "2026-02-10"^^xsd:date ;
        ] ;
.

:C2440
    a skos:Concept ;
    rdfs:isDefinedBy anzsic: ;
    skos:broader :C2400 ;
    skos:definition "An individual business entity whose predominant economic activity is Domestic Appliance Manufacturing."@en ;
    skos:inScheme cs: ;
    skos:notation "C2440" ;
    skos:prefLabel "Domestic Appliance Manufacturing"@en ;
    schema:temporalCoverage
        [
            schema:startTime "2026-02-10"^^xsd:date ;
        ] ;
.

:C2450
    a skos:Concept ;
    rdfs:isDefinedBy anzsic: ;
    skos:broader :C2400 ;
    skos:definition "An individual business entity whose predominant economic activity is Pump, Compressor, Heating and Ventilation Equipment Manufacturing."@en ;
    skos:inScheme cs: ;
    skos:notation "C2450" ;
    skos:prefLabel "Pump, Compressor, Heating and Ventilation Equipment Manufacturing"@en ;
    schema:temporalCoverage
        [
            schema:startTime "2026-02-10"^^xsd:date ;
        ] ;
.

:C2460
    a skos:Concept ;
    rdfs:isDefinedBy anzsic: ;
    skos:broader :C2400 ;
    skos:definition "An individual business entity whose predominant economic activity is Specialised Machinery and Equipment Manufacturing."@en ;
    skos:inScheme cs: ;
    skos:notation "C2460" ;
    skos:prefLabel "Specialised Machinery and Equipment Manufacturing"@en ;
    schema:temporalCoverage
        [
            schema:startTime "2026-02-10"^^xsd:date ;
        ] ;
.

:C2490
    a skos:Concept ;
    rdfs:isDefinedBy anzsic: ;
    skos:broader :C2400 ;
    skos:definition "An individual business entity whose predominant economic activity is Other Machinery and Equipment Manufacturing."@en ;
    skos:inScheme cs: ;
    skos:notation "C2490" ;
    skos:prefLabel "Other Machinery and Equipment Manufacturing"@en ;
    schema:temporalCoverage
        [
            schema:startTime "2026-02-10"^^xsd:date ;
        ] ;
.

:C2510
    a skos:Concept ;
    rdfs:isDefinedBy anzsic: ;
    skos:broader :C2500 ;
    skos:definition "An individual business entity whose predominant economic activity is Furniture Manufacturing."@en ;
    skos:inScheme cs: ;
    skos:notation "C2510" ;
    skos:prefLabel "Furniture Manufacturing"@en ;
    schema:temporalCoverage
        [
            schema:startTime "2026-02-10"^^xsd:date ;
        ] ;
.

:C2590
    a skos:Concept ;
    rdfs:isDefinedBy anzsic: ;
    skos:broader :C2500 ;
    skos:definition "An individual business entity whose predominant economic activity is Other Manufacturing."@en ;
    skos:inScheme cs: ;
    skos:notation "C2590" ;
    skos:prefLabel "Other Manufacturing"@en ;
    schema:temporalCoverage
        [
            schema:startTime "2026-02-10"^^xsd:date ;
        ] ;
.

:D2610
    a skos:Concept ;
    rdfs:isDefinedBy anzsic: ;
    skos:broader :D2600 ;
    skos:definition "An individual business entity whose predominant economic activity is Electricity Generation."@en ;
    skos:inScheme cs: ;
    skos:notation "D2610" ;
    skos:prefLabel "Electricity Generation"@en ;
    schema:temporalCoverage
        [
            schema:startTime "2026-02-10"^^xsd:date ;
        ] ;
.

:D2620
    a skos:Concept ;
    rdfs:isDefinedBy anzsic: ;
    skos:broader :D2600 ;
    skos:definition "An individual business entity whose predominant economic activity is Electricity Transmission."@en ;
    skos:inScheme cs: ;
    skos:notation "D2620" ;
    skos:prefLabel "Electricity Transmission"@en ;
    schema:temporalCoverage
        [
            schema:startTime "2026-02-10"^^xsd:date ;
        ] ;
.

:D2630
    a skos:Concept ;
    rdfs:isDefinedBy anzsic: ;
    skos:broader :D2600 ;
    skos:definition "An individual business entity whose predominant economic activity is Electricity Distribution."@en ;
    skos:inScheme cs: ;
    skos:notation "D2630" ;
    skos:prefLabel "Electricity Distribution"@en ;
    schema:temporalCoverage
        [
            schema:startTime "2026-02-10"^^xsd:date ;
        ] ;
.

:D2640
    a skos:Concept ;
    rdfs:isDefinedBy anzsic: ;
    skos:broader :D2600 ;
    skos:definition "An individual business entity whose predominant economic activity is On Selling Electricity and Electricity Market Operation."@en ;
    skos:inScheme cs: ;
    skos:notation "D2640" ;
    skos:prefLabel "On Selling Electricity and Electricity Market Operation"@en ;
    schema:temporalCoverage
        [
            schema:startTime "2026-02-10"^^xsd:date ;
        ] ;
.

:D2700
    a skos:Concept ;
    rdfs:isDefinedBy anzsic: ;
    skos:broader :D0000 ;
    skos:definition "An individual business entity whose predominant economic activity is Gas Supply."@en ;
    skos:inScheme cs: ;
    skos:notation "D2700" ;
    skos:prefLabel "Gas Supply"@en ;
    schema:temporalCoverage
        [
            schema:startTime "2026-02-10"^^xsd:date ;
        ] ;
.

:D2800
    a skos:Concept ;
    rdfs:isDefinedBy anzsic: ;
    skos:broader :D0000 ;
    skos:definition "An individual business entity whose predominant economic activity is Water Supply, Sewerage and Drainage Services."@en ;
    skos:inScheme cs: ;
    skos:notation "D2800" ;
    skos:prefLabel "Water Supply, Sewerage and Drainage Services"@en ;
    schema:temporalCoverage
        [
            schema:startTime "2026-02-10"^^xsd:date ;
        ] ;
.

:D2910
    a skos:Concept ;
    rdfs:isDefinedBy anzsic: ;
    skos:broader :D2900 ;
    skos:definition "An individual business entity whose predominant economic activity is Waste Collection Services."@en ;
    skos:inScheme cs: ;
    skos:notation "D2910" ;
    skos:prefLabel "Waste Collection Services"@en ;
    schema:temporalCoverage
        [
            schema:startTime "2026-02-10"^^xsd:date ;
        ] ;
.

:D2920
    a skos:Concept ;
    rdfs:isDefinedBy anzsic: ;
    skos:broader :D2900 ;
    skos:definition "An individual business entity whose predominant economic activity is Waste Treatment, Disposal and Remediation Services."@en ;
    skos:inScheme cs: ;
    skos:notation "D2920" ;
    skos:prefLabel "Waste Treatment, Disposal and Remediation Services"@en ;
    schema:temporalCoverage
        [
            schema:startTime "2026-02-10"^^xsd:date ;
        ] ;
.

:E3010
    a skos:Concept ;
    rdfs:isDefinedBy anzsic: ;
    skos:broader :E3000 ;
    skos:definition "An individual business entity whose predominant economic activity is Residential Building Construction."@en ;
    skos:inScheme cs: ;
    skos:notation "E3010" ;
    skos:prefLabel "Residential Building Construction"@en ;
    schema:temporalCoverage
        [
            schema:startTime "2026-02-10"^^xsd:date ;
        ] ;
.

:E3020
    a skos:Concept ;
    rdfs:isDefinedBy anzsic: ;
    skos:broader :E3000 ;
    skos:definition "An individual business entity whose predominant economic activity is Non-Residential Building Construction."@en ;
    skos:inScheme cs: ;
    skos:notation "E3020" ;
    skos:prefLabel "Non-Residential Building Construction"@en ;
    schema:temporalCoverage
        [
            schema:startTime "2026-02-10"^^xsd:date ;
        ] ;
.

:E3100
    a skos:Concept ;
    rdfs:isDefinedBy anzsic: ;
    skos:broader :E0000 ;
    skos:definition "An individual business entity whose predominant economic activity is Heavy and Civil Engineering Construction."@en ;
    skos:inScheme cs: ;
    skos:notation "E3100" ;
    skos:prefLabel "Heavy and Civil Engineering Construction"@en ;
    schema:temporalCoverage
        [
            schema:startTime "2026-02-10"^^xsd:date ;
        ] ;
.

:E3210
    a skos:Concept ;
    rdfs:isDefinedBy anzsic: ;
    skos:broader :E3200 ;
    skos:definition "An individual business entity whose predominant economic activity is Land Development and Site Preparation Services."@en ;
    skos:inScheme cs: ;
    skos:notation "E3210" ;
    skos:prefLabel "Land Development and Site Preparation Services"@en ;
    schema:temporalCoverage
        [
            schema:startTime "2026-02-10"^^xsd:date ;
        ] ;
.

:E3220
    a skos:Concept ;
    rdfs:isDefinedBy anzsic: ;
    skos:broader :E3200 ;
    skos:definition "An individual business entity whose predominant economic activity is Building Structure Services."@en ;
    skos:inScheme cs: ;
    skos:notation "E3220" ;
    skos:prefLabel "Building Structure Services"@en ;
    schema:temporalCoverage
        [
            schema:startTime "2026-02-10"^^xsd:date ;
        ] ;
.

:E3230
    a skos:Concept ;
    rdfs:isDefinedBy anzsic: ;
    skos:broader :E3200 ;
    skos:definition "An individual business entity whose predominant economic activity is Building Installation Services."@en ;
    skos:inScheme cs: ;
    skos:notation "E3230" ;
    skos:prefLabel "Building Installation Services"@en ;
    schema:temporalCoverage
        [
            schema:startTime "2026-02-10"^^xsd:date ;
        ] ;
.

:E3240
    a skos:Concept ;
    rdfs:isDefinedBy anzsic: ;
    skos:broader :E3200 ;
    skos:definition "An individual business entity whose predominant economic activity is Building Completion Services."@en ;
    skos:inScheme cs: ;
    skos:notation "E3240" ;
    skos:prefLabel "Building Completion Services"@en ;
    schema:temporalCoverage
        [
            schema:startTime "2026-02-10"^^xsd:date ;
        ] ;
.

:E3290
    a skos:Concept ;
    rdfs:isDefinedBy anzsic: ;
    skos:broader :E3200 ;
    skos:definition "An individual business entity whose predominant economic activity is Other Construction Services."@en ;
    skos:inScheme cs: ;
    skos:notation "E3290" ;
    skos:prefLabel "Other Construction Services"@en ;
    schema:temporalCoverage
        [
            schema:startTime "2026-02-10"^^xsd:date ;
        ] ;
.

:F3310
    a skos:Concept ;
    rdfs:isDefinedBy anzsic: ;
    skos:broader :F3300 ;
    skos:definition "An individual business entity whose predominant economic activity is Agricultural Product Wholesaling."@en ;
    skos:inScheme cs: ;
    skos:notation "F3310" ;
    skos:prefLabel "Agricultural Product Wholesaling"@en ;
    schema:temporalCoverage
        [
            schema:startTime "2026-02-10"^^xsd:date ;
        ] ;
.

:F3320
    a skos:Concept ;
    rdfs:isDefinedBy anzsic: ;
    skos:broader :F3300 ;
    skos:definition "An individual business entity whose predominant economic activity is Mineral, Metal and Chemical Wholesaling."@en ;
    skos:inScheme cs: ;
    skos:notation "F3320" ;
    skos:prefLabel "Mineral, Metal and Chemical Wholesaling"@en ;
    schema:temporalCoverage
        [
            schema:startTime "2026-02-10"^^xsd:date ;
        ] ;
.

:F3330
    a skos:Concept ;
    rdfs:isDefinedBy anzsic: ;
    skos:broader :F3300 ;
    skos:definition "An individual business entity whose predominant economic activity is Timber and Hardware Goods Wholesaling."@en ;
    skos:inScheme cs: ;
    skos:notation "F3330" ;
    skos:prefLabel "Timber and Hardware Goods Wholesaling"@en ;
    schema:temporalCoverage
        [
            schema:startTime "2026-02-10"^^xsd:date ;
        ] ;
.

:F3410
    a skos:Concept ;
    rdfs:isDefinedBy anzsic: ;
    skos:broader :F3400 ;
    skos:definition "An individual business entity whose predominant economic activity is Specialised Industrial Machinery and Equipment Wholesaling."@en ;
    skos:inScheme cs: ;
    skos:notation "F3410" ;
    skos:prefLabel "Specialised Industrial Machinery and Equipment Wholesaling"@en ;
    schema:temporalCoverage
        [
            schema:startTime "2026-02-10"^^xsd:date ;
        ] ;
.

:F3490
    a skos:Concept ;
    rdfs:isDefinedBy anzsic: ;
    skos:broader :F3400 ;
    skos:definition "An individual business entity whose predominant economic activity is Other Machinery and Equipment Wholesaling."@en ;
    skos:inScheme cs: ;
    skos:notation "F3490" ;
    skos:prefLabel "Other Machinery and Equipment Wholesaling"@en ;
    schema:temporalCoverage
        [
            schema:startTime "2026-02-10"^^xsd:date ;
        ] ;
.

:F3500
    a skos:Concept ;
    rdfs:isDefinedBy anzsic: ;
    skos:broader :F0000 ;
    skos:definition "An individual business entity whose predominant economic activity is Motor Vehicle and Motor Vehicle Parts Wholesaling."@en ;
    skos:inScheme cs: ;
    skos:notation "F3500" ;
    skos:prefLabel "Motor Vehicle and Motor Vehicle Parts Wholesaling"@en ;
    schema:temporalCoverage
        [
            schema:startTime "2026-02-10"^^xsd:date ;
        ] ;
.

:F3600
    a skos:Concept ;
    rdfs:isDefinedBy anzsic: ;
    skos:broader :F0000 ;
    skos:definition "An individual business entity whose predominant economic activity is Grocery, Liquor and Tobacco Product Wholesaling."@en ;
    skos:inScheme cs: ;
    skos:notation "F3600" ;
    skos:prefLabel "Grocery, Liquor and Tobacco Product Wholesaling"@en ;
    schema:temporalCoverage
        [
            schema:startTime "2026-02-10"^^xsd:date ;
        ] ;
.

:F3710
    a skos:Concept ;
    rdfs:isDefinedBy anzsic: ;
    skos:broader :F3700 ;
    skos:definition "An individual business entity whose predominant economic activity is Textile, Clothing and Footwear Wholesaling."@en ;
    skos:inScheme cs: ;
    skos:notation "F3710" ;
    skos:prefLabel "Textile, Clothing and Footwear Wholesaling"@en ;
    schema:temporalCoverage
        [
            schema:startTime "2026-02-10"^^xsd:date ;
        ] ;
.

:F3720
    a skos:Concept ;
    rdfs:isDefinedBy anzsic: ;
    skos:broader :F3700 ;
    skos:definition "An individual business entity whose predominant economic activity is Pharmaceutical and Toiletry Goods Wholesaling."@en ;
    skos:inScheme cs: ;
    skos:notation "F3720" ;
    skos:prefLabel "Pharmaceutical and Toiletry Goods Wholesaling"@en ;
    schema:temporalCoverage
        [
            schema:startTime "2026-02-10"^^xsd:date ;
        ] ;
.

:F3730
    a skos:Concept ;
    rdfs:isDefinedBy anzsic: ;
    skos:broader :F3700 ;
    skos:definition "An individual business entity whose predominant economic activity is Furniture, Floor Covering and Other Goods Wholesaling."@en ;
    skos:inScheme cs: ;
    skos:notation "F3730" ;
    skos:prefLabel "Furniture, Floor Covering and Other Goods Wholesaling"@en ;
    schema:temporalCoverage
        [
            schema:startTime "2026-02-10"^^xsd:date ;
        ] ;
.

:F3800
    a skos:Concept ;
    rdfs:isDefinedBy anzsic: ;
    skos:broader :F0000 ;
    skos:definition "An individual business entity whose predominant economic activity is Commission-Based Wholesaling."@en ;
    skos:inScheme cs: ;
    skos:notation "F3800" ;
    skos:prefLabel "Commission-Based Wholesaling"@en ;
    schema:temporalCoverage
        [
            schema:startTime "2026-02-10"^^xsd:date ;
        ] ;
.

:G3910
    a skos:Concept ;
    rdfs:isDefinedBy anzsic: ;
    skos:broader :G3900 ;
    skos:definition "An individual business entity whose predominant economic activity is Motor Vehicle Retailing."@en ;
    skos:inScheme cs: ;
    skos:notation "G3910" ;
    skos:prefLabel "Motor Vehicle Retailing"@en ;
    schema:temporalCoverage
        [
            schema:startTime "2026-02-10"^^xsd:date ;
        ] ;
.

:G3920
    a skos:Concept ;
    rdfs:isDefinedBy anzsic: ;
    skos:broader :G3900 ;
    skos:definition "An individual business entity whose predominant economic activity is Motor Vehicle Parts and Tyre Retailing."@en ;
    skos:inScheme cs: ;
    skos:notation "G3920" ;
    skos:prefLabel "Motor Vehicle Parts and Tyre Retailing"@en ;
    schema:temporalCoverage
        [
            schema:startTime "2026-02-10"^^xsd:date ;
        ] ;
.

:G4000
    a skos:Concept ;
    rdfs:isDefinedBy anzsic: ;
    skos:broader :G0000 ;
    skos:definition "An individual business entity whose predominant economic activity is Fuel Retailing."@en ;
    skos:inScheme cs: ;
    skos:notation "G4000" ;
    skos:prefLabel "Fuel Retailing"@en ;
    schema:temporalCoverage
        [
            schema:startTime "2026-02-10"^^xsd:date ;
        ] ;
.

:G4110
    a skos:Concept ;
    rdfs:isDefinedBy anzsic: ;
    skos:broader :G4100 ;
    skos:definition "An individual business entity whose predominant economic activity is Supermarket and Grocery Stores."@en ;
    skos:inScheme cs: ;
    skos:notation "G4110" ;
    skos:prefLabel "Supermarket and Grocery Stores"@en ;
    schema:temporalCoverage
        [
            schema:startTime "2026-02-10"^^xsd:date ;
        ] ;
.

:G4120
    a skos:Concept ;
    rdfs:isDefinedBy anzsic: ;
    skos:broader :G4100 ;
    skos:definition "An individual business entity whose predominant economic activity is Specialised Food Retailing."@en ;
    skos:inScheme cs: ;
    skos:notation "G4120" ;
    skos:prefLabel "Specialised Food Retailing"@en ;
    schema:temporalCoverage
        [
            schema:startTime "2026-02-10"^^xsd:date ;
        ] ;
.

:G4210
    a skos:Concept ;
    rdfs:isDefinedBy anzsic: ;
    skos:broader :G4200 ;
    skos:definition "An individual business entity whose predominant economic activity is Furniture, Floor Coverings, Houseware and Textile Goods Retailing."@en ;
    skos:inScheme cs: ;
    skos:notation "G4210" ;
    skos:prefLabel "Furniture, Floor Coverings, Houseware and Textile Goods Retailing"@en ;
    schema:temporalCoverage
        [
            schema:startTime "2026-02-10"^^xsd:date ;
        ] ;
.

:G4220
    a skos:Concept ;
    rdfs:isDefinedBy anzsic: ;
    skos:broader :G4200 ;
    skos:definition "An individual business entity whose predominant economic activity is Electrical and Electronic Goods Retailing."@en ;
    skos:inScheme cs: ;
    skos:notation "G4220" ;
    skos:prefLabel "Electrical and Electronic Goods Retailing"@en ;
    schema:temporalCoverage
        [
            schema:startTime "2026-02-10"^^xsd:date ;
        ] ;
.

:G4230
    a skos:Concept ;
    rdfs:isDefinedBy anzsic: ;
    skos:broader :G4200 ;
    skos:definition "An individual business entity whose predominant economic activity is Hardware, Building and Garden Supplies Retailing."@en ;
    skos:inScheme cs: ;
    skos:notation "G4230" ;
    skos:prefLabel "Hardware, Building and Garden Supplies Retailing"@en ;
    schema:temporalCoverage
        [
            schema:startTime "2026-02-10"^^xsd:date ;
        ] ;
.

:G4240
    a skos:Concept ;
    rdfs:isDefinedBy anzsic: ;
    skos:broader :G4200 ;
    skos:definition "An individual business entity whose predominant economic activity is Recreational Goods Retailing."@en ;
    skos:inScheme cs: ;
    skos:notation "G4240" ;
    skos:prefLabel "Recreational Goods Retailing"@en ;
    schema:temporalCoverage
        [
            schema:startTime "2026-02-10"^^xsd:date ;
        ] ;
.

:G4250
    a skos:Concept ;
    rdfs:isDefinedBy anzsic: ;
    skos:broader :G4200 ;
    skos:definition "An individual business entity whose predominant economic activity is Clothing, Footwear and Personal Accessory Retailing."@en ;
    skos:inScheme cs: ;
    skos:notation "G4250" ;
    skos:prefLabel "Clothing, Footwear and Personal Accessory Retailing"@en ;
    schema:temporalCoverage
        [
            schema:startTime "2026-02-10"^^xsd:date ;
        ] ;
.

:G4260
    a skos:Concept ;
    rdfs:isDefinedBy anzsic: ;
    skos:broader :G4200 ;
    skos:definition "An individual business entity whose predominant economic activity is Department Stores."@en ;
    skos:inScheme cs: ;
    skos:notation "G4260" ;
    skos:prefLabel "Department Stores"@en ;
    schema:temporalCoverage
        [
            schema:startTime "2026-02-10"^^xsd:date ;
        ] ;
.

:G4270
    a skos:Concept ;
    rdfs:isDefinedBy anzsic: ;
    skos:broader :G4200 ;
    skos:definition "An individual business entity whose predominant economic activity is Pharmaceutical and Other Store-Based Retailing."@en ;
    skos:inScheme cs: ;
    skos:notation "G4270" ;
    skos:prefLabel "Pharmaceutical and Other Store-Based Retailing"@en ;
    schema:temporalCoverage
        [
            schema:startTime "2026-02-10"^^xsd:date ;
        ] ;
.

:G4310
    a skos:Concept ;
    rdfs:isDefinedBy anzsic: ;
    skos:broader :G4300 ;
    skos:definition "An individual business entity whose predominant economic activity is Non-Store Retailing."@en ;
    skos:inScheme cs: ;
    skos:notation "G4310" ;
    skos:prefLabel "Non-Store Retailing"@en ;
    schema:temporalCoverage
        [
            schema:startTime "2026-02-10"^^xsd:date ;
        ] ;
.

:G4320
    a skos:Concept ;
    rdfs:isDefinedBy anzsic: ;
    skos:broader :G4300 ;
    skos:definition "An individual business entity whose predominant economic activity is Retail Commission-Based Buying and/or Selling."@en ;
    skos:inScheme cs: ;
    skos:notation "G4320" ;
    skos:prefLabel "Retail Commission-Based Buying and/or Selling"@en ;
    schema:temporalCoverage
        [
            schema:startTime "2026-02-10"^^xsd:date ;
        ] ;
.

:H4400
    a skos:Concept ;
    rdfs:isDefinedBy anzsic: ;
    skos:broader :H0000 ;
    skos:definition "An individual business entity whose predominant economic activity is Accommodation."@en ;
    skos:inScheme cs: ;
    skos:notation "H4400" ;
    skos:prefLabel "Accommodation"@en ;
    schema:temporalCoverage
        [
            schema:startTime "2026-02-10"^^xsd:date ;
        ] ;
.

:H4510
    a skos:Concept ;
    rdfs:isDefinedBy anzsic: ;
    skos:broader :H4500 ;
    skos:definition "An individual business entity whose predominant economic activity is Cafes, Restaurants and Takeaway Food Services."@en ;
    skos:inScheme cs: ;
    skos:notation "H4510" ;
    skos:prefLabel "Cafes, Restaurants and Takeaway Food Services"@en ;
    schema:temporalCoverage
        [
            schema:startTime "2026-02-10"^^xsd:date ;
        ] ;
.

:H4520
    a skos:Concept ;
    rdfs:isDefinedBy anzsic: ;
    skos:broader :H4500 ;
    skos:definition "An individual business entity whose predominant economic activity is Pubs, Taverns and Bars."@en ;
    skos:inScheme cs: ;
    skos:notation "H4520" ;
    skos:prefLabel "Pubs, Taverns and Bars"@en ;
    schema:temporalCoverage
        [
            schema:startTime "2026-02-10"^^xsd:date ;
        ] ;
.

:H4530
    a skos:Concept ;
    rdfs:isDefinedBy anzsic: ;
    skos:broader :H4500 ;
    skos:definition "An individual business entity whose predominant economic activity is Clubs (Hospitality)."@en ;
    skos:inScheme cs: ;
    skos:notation "H4530" ;
    skos:prefLabel "Clubs (Hospitality)"@en ;
    schema:temporalCoverage
        [
            schema:startTime "2026-02-10"^^xsd:date ;
        ] ;
.

:I4610
    a skos:Concept ;
    rdfs:isDefinedBy anzsic: ;
    skos:broader :I4600 ;
    skos:definition "An individual business entity whose predominant economic activity is Road Freight Transport."@en ;
    skos:inScheme cs: ;
    skos:notation "I4610" ;
    skos:prefLabel "Road Freight Transport"@en ;
    schema:temporalCoverage
        [
            schema:startTime "2026-02-10"^^xsd:date ;
        ] ;
.

:I4620
    a skos:Concept ;
    rdfs:isDefinedBy anzsic: ;
    skos:broader :I4600 ;
    skos:definition "An individual business entity whose predominant economic activity is Road Passenger Transport."@en ;
    skos:inScheme cs: ;
    skos:notation "I4620" ;
    skos:prefLabel "Road Passenger Transport"@en ;
    schema:temporalCoverage
        [
            schema:startTime "2026-02-10"^^xsd:date ;
        ] ;
.

:I4710
    a skos:Concept ;
    rdfs:isDefinedBy anzsic: ;
    skos:broader :I4700 ;
    skos:definition "An individual business entity whose predominant economic activity is Rail Freight Transport."@en ;
    skos:inScheme cs: ;
    skos:notation "I4710" ;
    skos:prefLabel "Rail Freight Transport"@en ;
    schema:temporalCoverage
        [
            schema:startTime "2026-02-10"^^xsd:date ;
        ] ;
.

:I4720
    a skos:Concept ;
    rdfs:isDefinedBy anzsic: ;
    skos:broader :I4700 ;
    skos:definition "An individual business entity whose predominant economic activity is Rail Passenger Transport."@en ;
    skos:inScheme cs: ;
    skos:notation "I4720" ;
    skos:prefLabel "Rail Passenger Transport"@en ;
    schema:temporalCoverage
        [
            schema:startTime "2026-02-10"^^xsd:date ;
        ] ;
.

:I4810
    a skos:Concept ;
    rdfs:isDefinedBy anzsic: ;
    skos:broader :I4800 ;
    skos:definition "An individual business entity whose predominant economic activity is Water Freight Transport."@en ;
    skos:inScheme cs: ;
    skos:notation "I4810" ;
    skos:prefLabel "Water Freight Transport"@en ;
    schema:temporalCoverage
        [
            schema:startTime "2026-02-10"^^xsd:date ;
        ] ;
.

:I4820
    a skos:Concept ;
    rdfs:isDefinedBy anzsic: ;
    skos:broader :I4800 ;
    skos:definition "An individual business entity whose predominant economic activity is Water Passenger Transport."@en ;
    skos:inScheme cs: ;
    skos:notation "I4820" ;
    skos:prefLabel "Water Passenger Transport"@en ;
    schema:temporalCoverage
        [
            schema:startTime "2026-02-10"^^xsd:date ;
        ] ;
.

:I4900
    a skos:Concept ;
    rdfs:isDefinedBy anzsic: ;
    skos:broader :I0000 ;
    skos:definition "An individual business entity whose predominant economic activity is Air and Space Transport."@en ;
    skos:inScheme cs: ;
    skos:notation "I4900" ;
    skos:prefLabel "Air and Space Transport"@en ;
    schema:temporalCoverage
        [
            schema:startTime "2026-02-10"^^xsd:date ;
        ] ;
.

:I5010
    a skos:Concept ;
    rdfs:isDefinedBy anzsic: ;
    skos:broader :I5000 ;
    skos:definition "An individual business entity whose predominant economic activity is Scenic and Sightseeing Transport."@en ;
    skos:inScheme cs: ;
    skos:notation "I5010" ;
    skos:prefLabel "Scenic and Sightseeing Transport"@en ;
    schema:temporalCoverage
        [
            schema:startTime "2026-02-10"^^xsd:date ;
        ] ;
.

:I5020
    a skos:Concept ;
    rdfs:isDefinedBy anzsic: ;
    skos:broader :I5000 ;
    skos:definition "An individual business entity whose predominant economic activity is Pipeline and Other Transport."@en ;
    skos:inScheme cs: ;
    skos:notation "I5020" ;
    skos:prefLabel "Pipeline and Other Transport"@en ;
    schema:temporalCoverage
        [
            schema:startTime "2026-02-10"^^xsd:date ;
        ] ;
.

:I5100
    a skos:Concept ;
    rdfs:isDefinedBy anzsic: ;
    skos:broader :I0000 ;
    skos:definition "An individual business entity whose predominant economic activity is Postal and Courier Pick-up and Delivery Services."@en ;
    skos:inScheme cs: ;
    skos:notation "I5100" ;
    skos:prefLabel "Postal and Courier Pick-up and Delivery Services"@en ;
    schema:temporalCoverage
        [
            schema:startTime "2026-02-10"^^xsd:date ;
        ] ;
.

:I5210
    a skos:Concept ;
    rdfs:isDefinedBy anzsic: ;
    skos:broader :I5200 ;
    skos:definition "An individual business entity whose predominant economic activity is Water Transport Support Services."@en ;
    skos:inScheme cs: ;
    skos:notation "I5210" ;
    skos:prefLabel "Water Transport Support Services"@en ;
    schema:temporalCoverage
        [
            schema:startTime "2026-02-10"^^xsd:date ;
        ] ;
.

:I5220
    a skos:Concept ;
    rdfs:isDefinedBy anzsic: ;
    skos:broader :I5200 ;
    skos:definition "An individual business entity whose predominant economic activity is Airport Operations and Other Air Transport Support Services."@en ;
    skos:inScheme cs: ;
    skos:notation "I5220" ;
    skos:prefLabel "Airport Operations and Other Air Transport Support Services"@en ;
    schema:temporalCoverage
        [
            schema:startTime "2026-02-10"^^xsd:date ;
        ] ;
.

:I5290
    a skos:Concept ;
    rdfs:isDefinedBy anzsic: ;
    skos:broader :I5200 ;
    skos:definition "An individual business entity whose predominant economic activity is Other Transport Support Services."@en ;
    skos:inScheme cs: ;
    skos:notation "I5290" ;
    skos:prefLabel "Other Transport Support Services"@en ;
    schema:temporalCoverage
        [
            schema:startTime "2026-02-10"^^xsd:date ;
        ] ;
.

:I5300
    a skos:Concept ;
    rdfs:isDefinedBy anzsic: ;
    skos:broader :I0000 ;
    skos:definition "An individual business entity whose predominant economic activity is Warehousing and Storage Services."@en ;
    skos:inScheme cs: ;
    skos:notation "I5300" ;
    skos:prefLabel "Warehousing and Storage Services"@en ;
    schema:temporalCoverage
        [
            schema:startTime "2026-02-10"^^xsd:date ;
        ] ;
.

:J5410
    a skos:Concept ;
    rdfs:isDefinedBy anzsic: ;
    skos:broader :J5400 ;
    skos:definition "An individual business entity whose predominant economic activity is Newspaper, Periodical, Book and Directory Publishing."@en ;
    skos:inScheme cs: ;
    skos:notation "J5410" ;
    skos:prefLabel "Newspaper, Periodical, Book and Directory Publishing"@en ;
    schema:temporalCoverage
        [
            schema:startTime "2026-02-10"^^xsd:date ;
        ] ;
.

:J5420
    a skos:Concept ;
    rdfs:isDefinedBy anzsic: ;
    skos:broader :J5400 ;
    skos:definition "An individual business entity whose predominant economic activity is Software Publishing."@en ;
    skos:inScheme cs: ;
    skos:notation "J5420" ;
    skos:prefLabel "Software Publishing"@en ;
    schema:temporalCoverage
        [
            schema:startTime "2026-02-10"^^xsd:date ;
        ] ;
.

:J5510
    a skos:Concept ;
    rdfs:isDefinedBy anzsic: ;
    skos:broader :J5500 ;
    skos:definition "An individual business entity whose predominant economic activity is Motion Picture and Video Activities."@en ;
    skos:inScheme cs: ;
    skos:notation "J5510" ;
    skos:prefLabel "Motion Picture and Video Activities"@en ;
    schema:temporalCoverage
        [
            schema:startTime "2026-02-10"^^xsd:date ;
        ] ;
.

:J5520
    a skos:Concept ;
    rdfs:isDefinedBy anzsic: ;
    skos:broader :J5500 ;
    skos:definition "An individual business entity whose predominant economic activity is Sound Recording and Music Publishing."@en ;
    skos:inScheme cs: ;
    skos:notation "J5520" ;
    skos:prefLabel "Sound Recording and Music Publishing"@en ;
    schema:temporalCoverage
        [
            schema:startTime "2026-02-10"^^xsd:date ;
        ] ;
.

:J5610
    a skos:Concept ;
    rdfs:isDefinedBy anzsic: ;
    skos:broader :J5600 ;
    skos:definition "An individual business entity whose predominant economic activity is Radio Broadcasting."@en ;
    skos:inScheme cs: ;
    skos:notation "J5610" ;
    skos:prefLabel "Radio Broadcasting"@en ;
    schema:temporalCoverage
        [
            schema:startTime "2026-02-10"^^xsd:date ;
        ] ;
.

:J5620
    a skos:Concept ;
    rdfs:isDefinedBy anzsic: ;
    skos:broader :J5600 ;
    skos:definition "An individual business entity whose predominant economic activity is Television Broadcasting."@en ;
    skos:inScheme cs: ;
    skos:notation "J5620" ;
    skos:prefLabel "Television Broadcasting"@en ;
    schema:temporalCoverage
        [
            schema:startTime "2026-02-10"^^xsd:date ;
        ] ;
.

:J5700
    a skos:Concept ;
    rdfs:isDefinedBy anzsic: ;
    skos:broader :J0000 ;
    skos:definition "An individual business entity whose predominant economic activity is Internet Publishing and Broadcasting."@en ;
    skos:inScheme cs: ;
    skos:notation "J5700" ;
    skos:prefLabel "Internet Publishing and Broadcasting"@en ;
    schema:temporalCoverage
        [
            schema:startTime "2026-02-10"^^xsd:date ;
        ] ;
.

:J5800
    a skos:Concept ;
    rdfs:isDefinedBy anzsic: ;
    skos:broader :J0000 ;
    skos:definition "An individual business entity whose predominant economic activity is Telecommunications Services."@en ;
    skos:inScheme cs: ;
    skos:notation "J5800" ;
    skos:prefLabel "Telecommunications Services"@en ;
    schema:temporalCoverage
        [
            schema:startTime "2026-02-10"^^xsd:date ;
        ] ;
.

:J5910
    a skos:Concept ;
    rdfs:isDefinedBy anzsic: ;
    skos:broader :J5900 ;
    skos:definition "An individual business entity whose predominant economic activity is Internet Service Providers and Web Search Portals."@en ;
    skos:inScheme cs: ;
    skos:notation "J5910" ;
    skos:prefLabel "Internet Service Providers and Web Search Portals"@en ;
    schema:temporalCoverage
        [
            schema:startTime "2026-02-10"^^xsd:date ;
        ] ;
.

:J5920
    a skos:Concept ;
    rdfs:isDefinedBy anzsic: ;
    skos:broader :J5900 ;
    skos:definition "An individual business entity whose predominant economic activity is Data Processing, Web Hosting and Electronic Information Storage Services."@en ;
    skos:inScheme cs: ;
    skos:notation "J5920" ;
    skos:prefLabel "Data Processing, Web Hosting and Electronic Information Storage Services"@en ;
    schema:temporalCoverage
        [
            schema:startTime "2026-02-10"^^xsd:date ;
        ] ;
.

:J6010
    a skos:Concept ;
    rdfs:isDefinedBy anzsic: ;
    skos:broader :J6000 ;
    skos:definition "An individual business entity whose predominant economic activity is Libraries and Archives."@en ;
    skos:inScheme cs: ;
    skos:notation "J6010" ;
    skos:prefLabel "Libraries and Archives"@en ;
    schema:temporalCoverage
        [
            schema:startTime "2026-02-10"^^xsd:date ;
        ] ;
.

:J6020
    a skos:Concept ;
    rdfs:isDefinedBy anzsic: ;
    skos:broader :J6000 ;
    skos:definition "An individual business entity whose predominant economic activity is Other Information Services."@en ;
    skos:inScheme cs: ;
    skos:notation "J6020" ;
    skos:prefLabel "Other Information Services"@en ;
    schema:temporalCoverage
        [
            schema:startTime "2026-02-10"^^xsd:date ;
        ] ;
.

:K6210
    a skos:Concept ;
    rdfs:isDefinedBy anzsic: ;
    skos:broader :K6200 ;
    skos:definition "An individual business entity whose predominant economic activity is Central Banking."@en ;
    skos:inScheme cs: ;
    skos:notation "K6210" ;
    skos:prefLabel "Central Banking"@en ;
    schema:temporalCoverage
        [
            schema:startTime "2026-02-10"^^xsd:date ;
        ] ;
.

:K6220
    a skos:Concept ;
    rdfs:isDefinedBy anzsic: ;
    skos:broader :K6200 ;
    skos:definition "An individual business entity whose predominant economic activity is Depository Financial Intermediation."@en ;
    skos:inScheme cs: ;
    skos:notation "K6220" ;
    skos:prefLabel "Depository Financial Intermediation"@en ;
    schema:temporalCoverage
        [
            schema:startTime "2026-02-10"^^xsd:date ;
        ] ;
.

:K6230
    a skos:Concept ;
    rdfs:isDefinedBy anzsic: ;
    skos:broader :K6200 ;
    skos:definition "An individual business entity whose predominant economic activity is Non-Depository Financing."@en ;
    skos:inScheme cs: ;
    skos:notation "K6230" ;
    skos:prefLabel "Non-Depository Financing"@en ;
    schema:temporalCoverage
        [
            schema:startTime "2026-02-10"^^xsd:date ;
        ] ;
.

:K6240
    a skos:Concept ;
    rdfs:isDefinedBy anzsic: ;
    skos:broader :K6200 ;
    skos:definition "An individual business entity whose predominant economic activity is Financial Asset Investing."@en ;
    skos:inScheme cs: ;
    skos:notation "K6240" ;
    skos:prefLabel "Financial Asset Investing"@en ;
    schema:temporalCoverage
        [
            schema:startTime "2026-02-10"^^xsd:date ;
        ] ;
.

:K6310
    a skos:Concept ;
    rdfs:isDefinedBy anzsic: ;
    skos:broader :K6300 ;
    skos:definition "An individual business entity whose predominant economic activity is Life Insurance."@en ;
    skos:inScheme cs: ;
    skos:notation "K6310" ;
    skos:prefLabel "Life Insurance"@en ;
    schema:temporalCoverage
        [
            schema:startTime "2026-02-10"^^xsd:date ;
        ] ;
.

:K6320
    a skos:Concept ;
    rdfs:isDefinedBy anzsic: ;
    skos:broader :K6300 ;
    skos:definition "An individual business entity whose predominant economic activity is Health and General Insurance."@en ;
    skos:inScheme cs: ;
    skos:notation "K6320" ;
    skos:prefLabel "Health and General Insurance"@en ;
    schema:temporalCoverage
        [
            schema:startTime "2026-02-10"^^xsd:date ;
        ] ;
.

:K6330
    a skos:Concept ;
    rdfs:isDefinedBy anzsic: ;
    skos:broader :K6300 ;
    skos:definition "An individual business entity whose predominant economic activity is Superannuation Funds."@en ;
    skos:inScheme cs: ;
    skos:notation "K6330" ;
    skos:prefLabel "Superannuation Funds"@en ;
    schema:temporalCoverage
        [
            schema:startTime "2026-02-10"^^xsd:date ;
        ] ;
.

:K6410
    a skos:Concept ;
    rdfs:isDefinedBy anzsic: ;
    skos:broader :K6400 ;
    skos:definition "An individual business entity whose predominant economic activity is Auxiliary Finance and Investment Services."@en ;
    skos:inScheme cs: ;
    skos:notation "K6410" ;
    skos:prefLabel "Auxiliary Finance and Investment Services"@en ;
    schema:temporalCoverage
        [
            schema:startTime "2026-02-10"^^xsd:date ;
        ] ;
.

:K6420
    a skos:Concept ;
    rdfs:isDefinedBy anzsic: ;
    skos:broader :K6400 ;
    skos:definition "An individual business entity whose predominant economic activity is Auxiliary Insurance Services."@en ;
    skos:inScheme cs: ;
    skos:notation "K6420" ;
    skos:prefLabel "Auxiliary Insurance Services"@en ;
    schema:temporalCoverage
        [
            schema:startTime "2026-02-10"^^xsd:date ;
        ] ;
.

:L6610
    a skos:Concept ;
    rdfs:isDefinedBy anzsic: ;
    skos:broader :L6600 ;
    skos:definition "An individual business entity whose predominant economic activity is Motor Vehicle and Transport Equipment Rental and Hiring."@en ;
    skos:inScheme cs: ;
    skos:notation "L6610" ;
    skos:prefLabel "Motor Vehicle and Transport Equipment Rental and Hiring"@en ;
    schema:temporalCoverage
        [
            schema:startTime "2026-02-10"^^xsd:date ;
        ] ;
.

:L6620
    a skos:Concept ;
    rdfs:isDefinedBy anzsic: ;
    skos:broader :L6600 ;
    skos:definition "An individual business entity whose predominant economic activity is Farm Animal and Bloodstock Leasing."@en ;
    skos:inScheme cs: ;
    skos:notation "L6620" ;
    skos:prefLabel "Farm Animal and Bloodstock Leasing"@en ;
    schema:temporalCoverage
        [
            schema:startTime "2026-02-10"^^xsd:date ;
        ] ;
.

:L6630
    a skos:Concept ;
    rdfs:isDefinedBy anzsic: ;
    skos:broader :L6600 ;
    skos:definition "An individual business entity whose predominant economic activity is Other Goods and Equipment Rental and Hiring."@en ;
    skos:inScheme cs: ;
    skos:notation "L6630" ;
    skos:prefLabel "Other Goods and Equipment Rental and Hiring"@en ;
    schema:temporalCoverage
        [
            schema:startTime "2026-02-10"^^xsd:date ;
        ] ;
.

:L6640
    a skos:Concept ;
    rdfs:isDefinedBy anzsic: ;
    skos:broader :L6600 ;
    skos:definition "An individual business entity whose predominant economic activity is Non-Financial Intangible Assets (Except Copyrights) Leasing."@en ;
    skos:inScheme cs: ;
    skos:notation "L6640" ;
    skos:prefLabel "Non-Financial Intangible Assets (Except Copyrights) Leasing"@en ;
    schema:temporalCoverage
        [
            schema:startTime "2026-02-10"^^xsd:date ;
        ] ;
.

:L6710
    a skos:Concept ;
    rdfs:isDefinedBy anzsic: ;
    skos:broader :L6700 ;
    skos:definition "An individual business entity whose predominant economic activity is Property Operators."@en ;
    skos:inScheme cs: ;
    skos:notation "L6710" ;
    skos:prefLabel "Property Operators"@en ;
    schema:temporalCoverage
        [
            schema:startTime "2026-02-10"^^xsd:date ;
        ] ;
.

:L6720
    a skos:Concept ;
    rdfs:isDefinedBy anzsic: ;
    skos:broader :L6700 ;
    skos:definition "An individual business entity whose predominant economic activity is Real Estate Services."@en ;
    skos:inScheme cs: ;
    skos:notation "L6720" ;
    skos:prefLabel "Real Estate Services"@en ;
    schema:temporalCoverage
        [
            schema:startTime "2026-02-10"^^xsd:date ;
        ] ;
.

:M6910
    a skos:Concept ;
    rdfs:isDefinedBy anzsic: ;
    skos:broader :M6900 ;
    skos:definition "An individual business entity whose predominant economic activity is Scientific Research Services."@en ;
    skos:inScheme cs: ;
    skos:notation "M6910" ;
    skos:prefLabel "Scientific Research Services"@en ;
    schema:temporalCoverage
        [
            schema:startTime "2026-02-10"^^xsd:date ;
        ] ;
.

:M6920
    a skos:Concept ;
    rdfs:isDefinedBy anzsic: ;
    skos:broader :M6900 ;
    skos:definition "An individual business entity whose predominant economic activity is Architectural, Engineering and Technical Services."@en ;
    skos:inScheme cs: ;
    skos:notation "M6920" ;
    skos:prefLabel "Architectural, Engineering and Technical Services"@en ;
    schema:temporalCoverage
        [
            schema:startTime "2026-02-10"^^xsd:date ;
        ] ;
.

:M6930
    a skos:Concept ;
    rdfs:isDefinedBy anzsic: ;
    skos:broader :M6900 ;
    skos:definition "An individual business entity whose predominant economic activity is Legal and Accounting Services."@en ;
    skos:inScheme cs: ;
    skos:notation "M6930" ;
    skos:prefLabel "Legal and Accounting Services"@en ;
    schema:temporalCoverage
        [
            schema:startTime "2026-02-10"^^xsd:date ;
        ] ;
.

:M6940
    a skos:Concept ;
    rdfs:isDefinedBy anzsic: ;
    skos:broader :M6900 ;
    skos:definition "An individual business entity whose predominant economic activity is Advertising Services."@en ;
    skos:inScheme cs: ;
    skos:notation "M6940" ;
    skos:prefLabel "Advertising Services"@en ;
    schema:temporalCoverage
        [
            schema:startTime "2026-02-10"^^xsd:date ;
        ] ;
.

:M6950
    a skos:Concept ;
    rdfs:isDefinedBy anzsic: ;
    skos:broader :M6900 ;
    skos:definition "An individual business entity whose predominant economic activity is Market Research and Statistical Services."@en ;
    skos:inScheme cs: ;
    skos:notation "M6950" ;
    skos:prefLabel "Market Research and Statistical Services"@en ;
    schema:temporalCoverage
        [
            schema:startTime "2026-02-10"^^xsd:date ;
        ] ;
.

:M6960
    a skos:Concept ;
    rdfs:isDefinedBy anzsic: ;
    skos:broader :M6900 ;
    skos:definition "An individual business entity whose predominant economic activity is Management and Related Consulting Services."@en ;
    skos:inScheme cs: ;
    skos:notation "M6960" ;
    skos:prefLabel "Management and Related Consulting Services"@en ;
    schema:temporalCoverage
        [
            schema:startTime "2026-02-10"^^xsd:date ;
        ] ;
.

:M6970
    a skos:Concept ;
    rdfs:isDefinedBy anzsic: ;
    skos:broader :M6900 ;
    skos:definition "An individual business entity whose predominant economic activity is Veterinary Services."@en ;
    skos:inScheme cs: ;
    skos:notation "M6970" ;
    skos:prefLabel "Veterinary Services"@en ;
    schema:temporalCoverage
        [
            schema:startTime "2026-02-10"^^xsd:date ;
        ] ;
.

:M6990
    a skos:Concept ;
    rdfs:isDefinedBy anzsic: ;
    skos:broader :M6900 ;
    skos:definition "An individual business entity whose predominant economic activity is Other Professional, Scientific and Technical Services."@en ;
    skos:inScheme cs: ;
    skos:notation "M6990" ;
    skos:prefLabel "Other Professional, Scientific and Technical Services"@en ;
    schema:temporalCoverage
        [
            schema:startTime "2026-02-10"^^xsd:date ;
        ] ;
.

:M7000
    a skos:Concept ;
    rdfs:isDefinedBy anzsic: ;
    skos:broader :M0000 ;
    skos:definition "An individual business entity whose predominant economic activity is Computer System Design and Related Services."@en ;
    skos:inScheme cs: ;
    skos:notation "M7000" ;
    skos:prefLabel "Computer System Design and Related Services"@en ;
    schema:temporalCoverage
        [
            schema:startTime "2026-02-10"^^xsd:date ;
        ] ;
.

:N7210
    a skos:Concept ;
    rdfs:isDefinedBy anzsic: ;
    skos:broader :N7200 ;
    skos:definition "An individual business entity whose predominant economic activity is Employment Services."@en ;
    skos:inScheme cs: ;
    skos:notation "N7210" ;
    skos:prefLabel "Employment Services"@en ;
    schema:temporalCoverage
        [
            schema:startTime "2026-02-10"^^xsd:date ;
        ] ;
.

:N7220
    a skos:Concept ;
    rdfs:isDefinedBy anzsic: ;
    skos:broader :N7200 ;
    skos:definition "An individual business entity whose predominant economic activity is Travel Agency and Tour Arrangement Services."@en ;
    skos:inScheme cs: ;
    skos:notation "N7220" ;
    skos:prefLabel "Travel Agency and Tour Arrangement Services"@en ;
    schema:temporalCoverage
        [
            schema:startTime "2026-02-10"^^xsd:date ;
        ] ;
.

:N7290
    a skos:Concept ;
    rdfs:isDefinedBy anzsic: ;
    skos:broader :N7200 ;
    skos:definition "An individual business entity whose predominant economic activity is Other Administrative Services."@en ;
    skos:inScheme cs: ;
    skos:notation "N7290" ;
    skos:prefLabel "Other Administrative Services"@en ;
    schema:temporalCoverage
        [
            schema:startTime "2026-02-10"^^xsd:date ;
        ] ;
.

:N7310
    a skos:Concept ;
    rdfs:isDefinedBy anzsic: ;
    skos:broader :N7300 ;
    skos:definition "An individual business entity whose predominant economic activity is Building Cleaning, Pest Control and Gardening Services."@en ;
    skos:inScheme cs: ;
    skos:notation "N7310" ;
    skos:prefLabel "Building Cleaning, Pest Control and Gardening Services"@en ;
    schema:temporalCoverage
        [
            schema:startTime "2026-02-10"^^xsd:date ;
        ] ;
.

:N7320
    a skos:Concept ;
    rdfs:isDefinedBy anzsic: ;
    skos:broader :N7300 ;
    skos:definition "An individual business entity whose predominant economic activity is Packaging Services."@en ;
    skos:inScheme cs: ;
    skos:notation "N7320" ;
    skos:prefLabel "Packaging Services"@en ;
    schema:temporalCoverage
        [
            schema:startTime "2026-02-10"^^xsd:date ;
        ] ;
.

:O7510
    a skos:Concept ;
    rdfs:isDefinedBy anzsic: ;
    skos:broader :O7500 ;
    skos:definition "An individual business entity whose predominant economic activity is Central Government Administration."@en ;
    skos:inScheme cs: ;
    skos:notation "O7510" ;
    skos:prefLabel "Central Government Administration"@en ;
    schema:temporalCoverage
        [
            schema:startTime "2026-02-10"^^xsd:date ;
        ] ;
.

:O7520
    a skos:Concept ;
    rdfs:isDefinedBy anzsic: ;
    skos:broader :O7500 ;
    skos:definition "An individual business entity whose predominant economic activity is State Government Administration."@en ;
    skos:inScheme cs: ;
    skos:notation "O7520" ;
    skos:prefLabel "State Government Administration"@en ;
    schema:temporalCoverage
        [
            schema:startTime "2026-02-10"^^xsd:date ;
        ] ;
.

:O7530
    a skos:Concept ;
    rdfs:isDefinedBy anzsic: ;
    skos:broader :O7500 ;
    skos:definition "An individual business entity whose predominant economic activity is Local Government Administration."@en ;
    skos:inScheme cs: ;
    skos:notation "O7530" ;
    skos:prefLabel "Local Government Administration"@en ;
    schema:temporalCoverage
        [
            schema:startTime "2026-02-10"^^xsd:date ;
        ] ;
.

:O7540
    a skos:Concept ;
    rdfs:isDefinedBy anzsic: ;
    skos:broader :O7500 ;
    skos:definition "An individual business entity whose predominant economic activity is Justice."@en ;
    skos:inScheme cs: ;
    skos:notation "O7540" ;
    skos:prefLabel "Justice"@en ;
    schema:temporalCoverage
        [
            schema:startTime "2026-02-10"^^xsd:date ;
        ] ;
.

:O7550
    a skos:Concept ;
    rdfs:isDefinedBy anzsic: ;
    skos:broader :O7500 ;
    skos:definition "An individual business entity whose predominant economic activity is Government Representation."@en ;
    skos:inScheme cs: ;
    skos:notation "O7550" ;
    skos:prefLabel "Government Representation"@en ;
    schema:temporalCoverage
        [
            schema:startTime "2026-02-10"^^xsd:date ;
        ] ;
.

:O7600
    a skos:Concept ;
    rdfs:isDefinedBy anzsic: ;
    skos:broader :O0000 ;
    skos:definition "An individual business entity whose predominant economic activity is Defence."@en ;
    skos:inScheme cs: ;
    skos:notation "O7600" ;
    skos:prefLabel "Defence"@en ;
    schema:temporalCoverage
        [
            schema:startTime "2026-02-10"^^xsd:date ;
        ] ;
.

:O7710
    a skos:Concept ;
    rdfs:isDefinedBy anzsic: ;
    skos:broader :O7700 ;
    skos:definition "An individual business entity whose predominant economic activity is Public Order and Safety Services."@en ;
    skos:inScheme cs: ;
    skos:notation "O7710" ;
    skos:prefLabel "Public Order and Safety Services"@en ;
    schema:temporalCoverage
        [
            schema:startTime "2026-02-10"^^xsd:date ;
        ] ;
.

:O7720
    a skos:Concept ;
    rdfs:isDefinedBy anzsic: ;
    skos:broader :O7700 ;
    skos:definition "An individual business entity whose predominant economic activity is Regulatory Services."@en ;
    skos:inScheme cs: ;
    skos:notation "O7720" ;
    skos:prefLabel "Regulatory Services"@en ;
    schema:temporalCoverage
        [
            schema:startTime "2026-02-10"^^xsd:date ;
        ] ;
.

:P8010
    a skos:Concept ;
    rdfs:isDefinedBy anzsic: ;
    skos:broader :P8000 ;
    skos:definition "An individual business entity whose predominant economic activity is Preschool Education."@en ;
    skos:inScheme cs: ;
    skos:notation "P8010" ;
    skos:prefLabel "Preschool Education"@en ;
    schema:temporalCoverage
        [
            schema:startTime "2026-02-10"^^xsd:date ;
        ] ;
.

:P8020
    a skos:Concept ;
    rdfs:isDefinedBy anzsic: ;
    skos:broader :P8000 ;
    skos:definition "An individual business entity whose predominant economic activity is School Education."@en ;
    skos:inScheme cs: ;
    skos:notation "P8020" ;
    skos:prefLabel "School Education"@en ;
    schema:temporalCoverage
        [
            schema:startTime "2026-02-10"^^xsd:date ;
        ] ;
.

:P8100
    a skos:Concept ;
    rdfs:isDefinedBy anzsic: ;
    skos:broader :P0000 ;
    skos:definition "An individual business entity whose predominant economic activity is Tertiary Education."@en ;
    skos:inScheme cs: ;
    skos:notation "P8100" ;
    skos:prefLabel "Tertiary Education"@en ;
    schema:temporalCoverage
        [
            schema:startTime "2026-02-10"^^xsd:date ;
        ] ;
.

:P8220
    a skos:Concept ;
    rdfs:isDefinedBy anzsic: ;
    skos:broader :P8200 ;
    skos:definition "An individual business entity whose predominant economic activity is Educational Support Services."@en ;
    skos:inScheme cs: ;
    skos:notation "P8220" ;
    skos:prefLabel "Educational Support Services"@en ;
    schema:temporalCoverage
        [
            schema:startTime "2026-02-10"^^xsd:date ;
        ] ;
.

:Q8400
    a skos:Concept ;
    rdfs:isDefinedBy anzsic: ;
    skos:broader :Q0000 ;
    skos:definition "An individual business entity whose predominant economic activity is Hospitals."@en ;
    skos:inScheme cs: ;
    skos:notation "Q8400" ;
    skos:prefLabel "Hospitals"@en ;
    schema:temporalCoverage
        [
            schema:startTime "2026-02-10"^^xsd:date ;
        ] ;
.

:Q8510
    a skos:Concept ;
    rdfs:isDefinedBy anzsic: ;
    skos:broader :Q8500 ;
    skos:definition "An individual business entity whose predominant economic activity is Medical Services."@en ;
    skos:inScheme cs: ;
    skos:notation "Q8510" ;
    skos:prefLabel "Medical Services"@en ;
    schema:temporalCoverage
        [
            schema:startTime "2026-02-10"^^xsd:date ;
        ] ;
.

:Q8520
    a skos:Concept ;
    rdfs:isDefinedBy anzsic: ;
    skos:broader :Q8500 ;
    skos:definition "An individual business entity whose predominant economic activity is Pathology and Diagnostic Imaging Services."@en ;
    skos:inScheme cs: ;
    skos:notation "Q8520" ;
    skos:prefLabel "Pathology and Diagnostic Imaging Services"@en ;
    schema:temporalCoverage
        [
            schema:startTime "2026-02-10"^^xsd:date ;
        ] ;
.

:Q8530
    a skos:Concept ;
    rdfs:isDefinedBy anzsic: ;
    skos:broader :Q8500 ;
    skos:definition "An individual business entity whose predominant economic activity is Allied Health Services."@en ;
    skos:inScheme cs: ;
    skos:notation "Q8530" ;
    skos:prefLabel "Allied Health Services"@en ;
    schema:temporalCoverage
        [
            schema:startTime "2026-02-10"^^xsd:date ;
        ] ;
.

:Q8590
    a skos:Concept ;
    rdfs:isDefinedBy anzsic: ;
    skos:broader :Q8500 ;
    skos:definition "An individual business entity whose predominant economic activity is Other Health Care Services."@en ;
    skos:inScheme cs: ;
    skos:notation "Q8590" ;
    skos:prefLabel "Other Health Care Services"@en ;
    schema:temporalCoverage
        [
            schema:startTime "2026-02-10"^^xsd:date ;
        ] ;
.

:Q8600
    a skos:Concept ;
    rdfs:isDefinedBy anzsic: ;
    skos:broader :Q0000 ;
    skos:definition "An individual business entity whose predominant economic activity is Residential Care Services."@en ;
    skos:inScheme cs: ;
    skos:notation "Q8600" ;
    skos:prefLabel "Residential Care Services"@en ;
    schema:temporalCoverage
        [
            schema:startTime "2026-02-10"^^xsd:date ;
        ] ;
.

:Q8710
    a skos:Concept ;
    rdfs:isDefinedBy anzsic: ;
    skos:broader :Q8700 ;
    skos:definition "An individual business entity whose predominant economic activity is Child Care Services."@en ;
    skos:inScheme cs: ;
    skos:notation "Q8710" ;
    skos:prefLabel "Child Care Services"@en ;
    schema:temporalCoverage
        [
            schema:startTime "2026-02-10"^^xsd:date ;
        ] ;
.

:Q8790
    a skos:Concept ;
    rdfs:isDefinedBy anzsic: ;
    skos:broader :Q8700 ;
    skos:definition "An individual business entity whose predominant economic activity is Other Social Assistance Services."@en ;
    skos:inScheme cs: ;
    skos:notation "Q8790" ;
    skos:prefLabel "Other Social Assistance Services"@en ;
    schema:temporalCoverage
        [
            schema:startTime "2026-02-10"^^xsd:date ;
        ] ;
.

:R8910
    a skos:Concept ;
    rdfs:isDefinedBy anzsic: ;
    skos:broader :R8900 ;
    skos:definition "An individual business entity whose predominant economic activity is Museum Operation."@en ;
    skos:inScheme cs: ;
    skos:notation "R8910" ;
    skos:prefLabel "Museum Operation"@en ;
    schema:temporalCoverage
        [
            schema:startTime "2026-02-10"^^xsd:date ;
        ] ;
.

:R8920
    a skos:Concept ;
    rdfs:isDefinedBy anzsic: ;
    skos:broader :R8900 ;
    skos:definition "An individual business entity whose predominant economic activity is Parks and Gardens Operations."@en ;
    skos:inScheme cs: ;
    skos:notation "R8920" ;
    skos:prefLabel "Parks and Gardens Operations"@en ;
    schema:temporalCoverage
        [
            schema:startTime "2026-02-10"^^xsd:date ;
        ] ;
.

:R9000
    a skos:Concept ;
    rdfs:isDefinedBy anzsic: ;
    skos:broader :R0000 ;
    skos:definition "An individual business entity whose predominant economic activity is Creative and Performing Arts Activities."@en ;
    skos:inScheme cs: ;
    skos:notation "R9000" ;
    skos:prefLabel "Creative and Performing Arts Activities"@en ;
    schema:temporalCoverage
        [
            schema:startTime "2026-02-10"^^xsd:date ;
        ] ;
.

:R9110
    a skos:Concept ;
    rdfs:isDefinedBy anzsic: ;
    skos:broader :R9100 ;
    skos:definition "An individual business entity whose predominant economic activity is Sports and Physical Recreation Activities."@en ;
    skos:inScheme cs: ;
    skos:notation "R9110" ;
    skos:prefLabel "Sports and Physical Recreation Activities"@en ;
    schema:temporalCoverage
        [
            schema:startTime "2026-02-10"^^xsd:date ;
        ] ;
.

:R9120
    a skos:Concept ;
    rdfs:isDefinedBy anzsic: ;
    skos:broader :R9100 ;
    skos:definition "An individual business entity whose predominant economic activity is Horse and Dog Racing Activities."@en ;
    skos:inScheme cs: ;
    skos:notation "R9120" ;
    skos:prefLabel "Horse and Dog Racing Activities"@en ;
    schema:temporalCoverage
        [
            schema:startTime "2026-02-10"^^xsd:date ;
        ] ;
.

:R9130
    a skos:Concept ;
    rdfs:isDefinedBy anzsic: ;
    skos:broader :R9100 ;
    skos:definition "An individual business entity whose predominant economic activity is Amusement and Other Recreation Activities."@en ;
    skos:inScheme cs: ;
    skos:notation "R9130" ;
    skos:prefLabel "Amusement and Other Recreation Activities"@en ;
    schema:temporalCoverage
        [
            schema:startTime "2026-02-10"^^xsd:date ;
        ] ;
.

:R9200
    a skos:Concept ;
    rdfs:isDefinedBy anzsic: ;
    skos:broader :R0000 ;
    skos:definition "An individual business entity whose predominant economic activity is Gambling Activities."@en ;
    skos:inScheme cs: ;
    skos:notation "R9200" ;
    skos:prefLabel "Gambling Activities"@en ;
    schema:temporalCoverage
        [
            schema:startTime "2026-02-10"^^xsd:date ;
        ] ;
.

:S9410
    a skos:Concept ;
    rdfs:isDefinedBy anzsic: ;
    skos:broader :S9400 ;
    skos:definition "An individual business entity whose predominant economic activity is Automotive Repair and Maintenance."@en ;
    skos:inScheme cs: ;
    skos:notation "S9410" ;
    skos:prefLabel "Automotive Repair and Maintenance"@en ;
    schema:temporalCoverage
        [
            schema:startTime "2026-02-10"^^xsd:date ;
        ] ;
.

:S9420
    a skos:Concept ;
    rdfs:isDefinedBy anzsic: ;
    skos:broader :S9400 ;
    skos:definition "An individual business entity whose predominant economic activity is Machinery and Equipment Repair and Maintenance."@en ;
    skos:inScheme cs: ;
    skos:notation "S9420" ;
    skos:prefLabel "Machinery and Equipment Repair and Maintenance"@en ;
    schema:temporalCoverage
        [
            schema:startTime "2026-02-10"^^xsd:date ;
        ] ;
.

:S9490
    a skos:Concept ;
    rdfs:isDefinedBy anzsic: ;
    skos:broader :S9400 ;
    skos:definition "An individual business entity whose predominant economic activity is Other Repair and Maintenance."@en ;
    skos:inScheme cs: ;
    skos:notation "S9490" ;
    skos:prefLabel "Other Repair and Maintenance"@en ;
    schema:temporalCoverage
        [
            schema:startTime "2026-02-10"^^xsd:date ;
        ] ;
.

:S9510
    a skos:Concept ;
    rdfs:isDefinedBy anzsic: ;
    skos:broader :S9500 ;
    skos:definition "An individual business entity whose predominant economic activity is Personal Care Services."@en ;
    skos:inScheme cs: ;
    skos:notation "S9510" ;
    skos:prefLabel "Personal Care Services"@en ;
    schema:temporalCoverage
        [
            schema:startTime "2026-02-10"^^xsd:date ;
        ] ;
.

:S9520
    a skos:Concept ;
    rdfs:isDefinedBy anzsic: ;
    skos:broader :S9500 ;
    skos:definition "An individual business entity whose predominant economic activity is Funeral, Crematorium and Cemetery Services."@en ;
    skos:inScheme cs: ;
    skos:notation "S9520" ;
    skos:prefLabel "Funeral, Crematorium and Cemetery Services"@en ;
    schema:temporalCoverage
        [
            schema:startTime "2026-02-10"^^xsd:date ;
        ] ;
.

:S9530
    a skos:Concept ;
    rdfs:isDefinedBy anzsic: ;
    skos:broader :S9500 ;
    skos:definition "An individual business entity whose predominant economic activity is Other Personal Services."@en ;
    skos:inScheme cs: ;
    skos:notation "S9530" ;
    skos:prefLabel "Other Personal Services"@en ;
    schema:temporalCoverage
        [
            schema:startTime "2026-02-10"^^xsd:date ;
        ] ;
.

:S9540
    a skos:Concept ;
    rdfs:isDefinedBy anzsic: ;
    skos:broader :S9500 ;
    skos:definition "An individual business entity whose predominant economic activity is Religious Services."@en ;
    skos:inScheme cs: ;
    skos:notation "S9540" ;
    skos:prefLabel "Religious Services"@en ;
    schema:temporalCoverage
        [
            schema:startTime "2026-02-10"^^xsd:date ;
        ] ;
.

:S9550
    a skos:Concept ;
    rdfs:isDefinedBy anzsic: ;
    skos:broader :S9500 ;
    skos:definition "An individual business entity whose predominant economic activity is Civic, Professional and Other Interest Group Services."@en ;
    skos:inScheme cs: ;
    skos:notation "S9550" ;
    skos:prefLabel "Civic, Professional and Other Interest Group Services"@en ;
    schema:temporalCoverage
        [
            schema:startTime "2026-02-10"^^xsd:date ;
        ] ;
.

:S9600
    a skos:Concept ;
    rdfs:isDefinedBy anzsic: ;
    skos:broader :S0000 ;
    skos:definition "An individual business entity whose predominant economic activity is Private Households Employing Staff and Undifferentiated Goods and Service Producing Activities of Households for Own Use."@en ;
    skos:inScheme cs: ;
    skos:notation "S9600" ;
    skos:prefLabel "Private Households Employing Staff and Undifferentiated Goods and Service Producing Activities of Households for Own Use"@en ;
    schema:temporalCoverage
        [
            schema:startTime "2026-02-10"^^xsd:date ;
        ] ;
.

:X9800
    a skos:Concept ;
    rdfs:isDefinedBy anzsic: ;
    skos:altLabel
        "Other"@en ,
        "Other Industry"@en ;
    skos:broader :X0000 ;
    skos:definition "An individual business entity whose predominant economic activity is unspecified or is not available for selection with provided list. This typically applies to a known industrial classification that is not relevant to a high degree of specificity in a specific use case."@en ;
    skos:inScheme cs: ;
    skos:notation "X9800" ;
    skos:prefLabel "Unspecified Industry"@en ;
    schema:temporalCoverage
        [
            schema:startTime "2026-02-10"^^xsd:date ;
        ] ;
.

:X9900
    a skos:Concept ;
    rdfs:isDefinedBy anzsic: ;
    skos:altLabel "Unknown Industry"@en ;
    skos:broader :X0000 ;
    skos:definition "An individual business entity whose predominant economic activity is unknown."@en ;
    skos:inScheme cs: ;
    skos:notation "X9900" ;
    skos:prefLabel "Unknown"@en ;
    schema:temporalCoverage
        [
            schema:startTime "2026-02-10"^^xsd:date ;
        ] ;
.

:C0000-2
    a skos:Concept ;
    dcterms:replaces :C0000 ;
    rdfs:isDefinedBy cs: ;
    skos:definition "An individual business entity whose predominant economic activity is Manufacturing of physical goods."@en ;
    skos:inScheme cs: ;
    skos:notation "C0000" ;
    skos:prefLabel "Manufacturing of goods"@en ;
    skos:topConceptOf cs: ;
    schema:temporalCoverage
        [
            schema:startTime "2026-02-12"^^xsd:date ;
        ] ;
    schema:creator <https://orcid.org/0000-0002-8742-7730> ;
.

:C1510
    a skos:Concept ;
    rdfs:isDefinedBy anzsic: ;
    skos:broader :C1500 ;
    skos:definition "An individual business entity whose predominant economic activity is Pulp, Paper and Paperboard Manufacturing."@en ;
    skos:inScheme cs: ;
    skos:notation "C1510" ;
    skos:prefLabel "Pulp, Paper and Paperboard Manufacturing"@en ;
    schema:temporalCoverage
        [
            schema:startTime "2026-02-10"^^xsd:date ;
        ] ;
.

:P8200
    a skos:Concept ;
    rdfs:isDefinedBy anzsic: ;
    skos:broader :P0000 ;
    skos:definition "An individual business entity whose predominant economic activity is Adult, Community and Other Education."@en ;
    skos:inScheme cs: ;
    skos:notation "P8200" ;
    skos:prefLabel "Adult, Community and Other Education"@en ;
    schema:temporalCoverage
        [
            schema:startTime "2026-02-10"^^xsd:date ;
        ] ;
.

:A0400
    a skos:Concept ;
    rdfs:isDefinedBy anzsic: ;
    skos:broader :A0000 ;
    skos:definition "An individual business entity whose predominant economic activity is Fishing, Hunting and Trapping."@en ;
    skos:inScheme cs: ;
    skos:notation "A0400" ;
    skos:prefLabel "Fishing, Hunting and Trapping"@en ;
    schema:temporalCoverage
        [
            schema:startTime "2026-02-10"^^xsd:date ;
        ] ;
.

:A0500
    a skos:Concept ;
    rdfs:isDefinedBy anzsic: ;
    skos:broader :A0000 ;
    skos:definition "An individual business entity whose predominant economic activity is Agriculture, Forestry and Fishing Support Services."@en ;
    skos:inScheme cs: ;
    skos:notation "A0500" ;
    skos:prefLabel "Agriculture, Forestry and Fishing Support Services"@en ;
    schema:temporalCoverage
        [
            schema:startTime "2026-02-10"^^xsd:date ;
        ] ;
.

:B0900
    a skos:Concept ;
    rdfs:isDefinedBy anzsic: ;
    skos:broader :B0000 ;
    skos:definition "An individual business entity whose predominant economic activity is Non-Metallic Mineral Mining and Quarrying."@en ;
    skos:inScheme cs: ;
    skos:notation "B0900" ;
    skos:prefLabel "Non-Metallic Mineral Mining and Quarrying"@en ;
    schema:temporalCoverage
        [
            schema:startTime "2026-02-10"^^xsd:date ;
        ] ;
.

:B1000
    a skos:Concept ;
    rdfs:isDefinedBy anzsic: ;
    skos:broader :B0000 ;
    skos:definition "An individual business entity whose predominant economic activity is Exploration and Other Mining Support Services."@en ;
    skos:inScheme cs: ;
    skos:notation "B1000" ;
    skos:prefLabel "Exploration and Other Mining Support Services"@en ;
    schema:temporalCoverage
        [
            schema:startTime "2026-02-10"^^xsd:date ;
        ] ;
.

:C1200
    a skos:Concept ;
    rdfs:isDefinedBy anzsic: ;
    skos:broader :C0000 ;
    skos:definition "An individual business entity whose predominant economic activity is Beverage and Tobacco Product Manufacturing."@en ;
    skos:inScheme cs: ;
    skos:notation "C1200" ;
    skos:prefLabel "Beverage and Tobacco Product Manufacturing"@en ;
    schema:temporalCoverage
        [
            schema:startTime "2026-02-10"^^xsd:date ;
        ] ;
.

:C1400
    a skos:Concept ;
    rdfs:isDefinedBy anzsic: ;
    skos:broader :C0000 ;
    skos:definition "An individual business entity whose predominant economic activity is Wood Product Manufacturing."@en ;
    skos:inScheme cs: ;
    skos:notation "C1400" ;
    skos:prefLabel "Wood Product Manufacturing"@en ;
    schema:temporalCoverage
        [
            schema:startTime "2026-02-10"^^xsd:date ;
        ] ;
.

:C1500
    a skos:Concept ;
    rdfs:isDefinedBy anzsic: ;
    skos:broader :C0000 ;
    skos:definition "An individual business entity whose predominant economic activity is Pulp, Paper and Converted Paper Product Manufacturing."@en ;
    skos:inScheme cs: ;
    skos:notation "C1500" ;
    skos:prefLabel "Pulp, Paper and Converted Paper Product Manufacturing"@en ;
    schema:temporalCoverage
        [
            schema:startTime "2026-02-10"^^xsd:date ;
        ] ;
.

:C1600
    a skos:Concept ;
    rdfs:isDefinedBy anzsic: ;
    skos:broader :C0000 ;
    skos:definition "An individual business entity whose predominant economic activity is Printing (including the Reproduction of Recorded Media)."@en ;
    skos:inScheme cs: ;
    skos:notation "C1600" ;
    skos:prefLabel "Printing (including the Reproduction of Recorded Media)"@en ;
    schema:temporalCoverage
        [
            schema:startTime "2026-02-10"^^xsd:date ;
        ] ;
.

:C1900
    a skos:Concept ;
    rdfs:isDefinedBy anzsic: ;
    skos:broader :C0000 ;
    skos:definition "An individual business entity whose predominant economic activity is Polymer Product and Rubber Product Manufacturing."@en ;
    skos:inScheme cs: ;
    skos:notation "C1900" ;
    skos:prefLabel "Polymer Product and Rubber Product Manufacturing"@en ;
    schema:temporalCoverage
        [
            schema:startTime "2026-02-10"^^xsd:date ;
        ] ;
.

:C2300
    a skos:Concept ;
    rdfs:isDefinedBy anzsic: ;
    skos:broader :C0000 ;
    skos:definition "An individual business entity whose predominant economic activity is Transport Equipment Manufacturing."@en ;
    skos:inScheme cs: ;
    skos:notation "C2300" ;
    skos:prefLabel "Transport Equipment Manufacturing"@en ;
    schema:temporalCoverage
        [
            schema:startTime "2026-02-10"^^xsd:date ;
        ] ;
.

:C2500
    a skos:Concept ;
    rdfs:isDefinedBy anzsic: ;
    skos:broader :C0000 ;
    skos:definition "An individual business entity whose predominant economic activity is Furniture and Other Manufacturing."@en ;
    skos:inScheme cs: ;
    skos:notation "C2500" ;
    skos:prefLabel "Furniture and Other Manufacturing"@en ;
    schema:temporalCoverage
        [
            schema:startTime "2026-02-10"^^xsd:date ;
        ] ;
.

:D2900
    a skos:Concept ;
    rdfs:isDefinedBy anzsic: ;
    skos:broader :D0000 ;
    skos:definition "An individual business entity whose predominant economic activity is Waste Collection, Treatment and Disposal Services."@en ;
    skos:inScheme cs: ;
    skos:notation "D2900" ;
    skos:prefLabel "Waste Collection, Treatment and Disposal Services"@en ;
    schema:temporalCoverage
        [
            schema:startTime "2026-02-10"^^xsd:date ;
        ] ;
.

:E3000
    a skos:Concept ;
    rdfs:isDefinedBy anzsic: ;
    skos:broader :E0000 ;
    skos:definition "An individual business entity whose predominant economic activity is Building Construction."@en ;
    skos:inScheme cs: ;
    skos:notation "E3000" ;
    skos:prefLabel "Building Construction"@en ;
    schema:temporalCoverage
        [
            schema:startTime "2026-02-10"^^xsd:date ;
        ] ;
.

:F3400
    a skos:Concept ;
    rdfs:isDefinedBy anzsic: ;
    skos:broader :F0000 ;
    skos:definition "An individual business entity whose predominant economic activity is Machinery and Equipment Wholesaling."@en ;
    skos:inScheme cs: ;
    skos:notation "F3400" ;
    skos:prefLabel "Machinery and Equipment Wholesaling"@en ;
    schema:temporalCoverage
        [
            schema:startTime "2026-02-10"^^xsd:date ;
        ] ;
.

:G3900
    a skos:Concept ;
    rdfs:isDefinedBy anzsic: ;
    skos:broader :G0000 ;
    skos:definition "An individual business entity whose predominant economic activity is Motor Vehicle and Motor Vehicle Parts Retailing."@en ;
    skos:inScheme cs: ;
    skos:notation "G3900" ;
    skos:prefLabel "Motor Vehicle and Motor Vehicle Parts Retailing"@en ;
    schema:temporalCoverage
        [
            schema:startTime "2026-02-10"^^xsd:date ;
        ] ;
.

:G4100
    a skos:Concept ;
    rdfs:isDefinedBy anzsic: ;
    skos:broader :G0000 ;
    skos:definition "An individual business entity whose predominant economic activity is Food Retailing."@en ;
    skos:inScheme cs: ;
    skos:notation "G4100" ;
    skos:prefLabel "Food Retailing"@en ;
    schema:temporalCoverage
        [
            schema:startTime "2026-02-10"^^xsd:date ;
        ] ;
.

:G4300
    a skos:Concept ;
    rdfs:isDefinedBy anzsic: ;
    skos:broader :G0000 ;
    skos:definition "An individual business entity whose predominant economic activity is Non-Store Retailing and Retail Commission-Based Buying and/or Selling."@en ;
    skos:inScheme cs: ;
    skos:notation "G4300" ;
    skos:prefLabel "Non-Store Retailing and Retail Commission-Based Buying and/or Selling"@en ;
    schema:temporalCoverage
        [
            schema:startTime "2026-02-10"^^xsd:date ;
        ] ;
.

:I4600
    a skos:Concept ;
    rdfs:isDefinedBy anzsic: ;
    skos:broader :I0000 ;
    skos:definition "An individual business entity whose predominant economic activity is Road Transport."@en ;
    skos:inScheme cs: ;
    skos:notation "I4600" ;
    skos:prefLabel "Road Transport"@en ;
    schema:temporalCoverage
        [
            schema:startTime "2026-02-10"^^xsd:date ;
        ] ;
.

:I4700
    a skos:Concept ;
    rdfs:isDefinedBy anzsic: ;
    skos:broader :I0000 ;
    skos:definition "An individual business entity whose predominant economic activity is Rail Transport."@en ;
    skos:inScheme cs: ;
    skos:notation "I4700" ;
    skos:prefLabel "Rail Transport"@en ;
    schema:temporalCoverage
        [
            schema:startTime "2026-02-10"^^xsd:date ;
        ] ;
.

:I4800
    a skos:Concept ;
    rdfs:isDefinedBy anzsic: ;
    skos:broader :I0000 ;
    skos:definition "An individual business entity whose predominant economic activity is Water Transport."@en ;
    skos:inScheme cs: ;
    skos:notation "I4800" ;
    skos:prefLabel "Water Transport"@en ;
    schema:temporalCoverage
        [
            schema:startTime "2026-02-10"^^xsd:date ;
        ] ;
.

:I5000
    a skos:Concept ;
    rdfs:isDefinedBy anzsic: ;
    skos:broader :I0000 ;
    skos:definition "An individual business entity whose predominant economic activity is Other Transport."@en ;
    skos:inScheme cs: ;
    skos:notation "I5000" ;
    skos:prefLabel "Other Transport"@en ;
    schema:temporalCoverage
        [
            schema:startTime "2026-02-10"^^xsd:date ;
        ] ;
.

:J5400
    a skos:Concept ;
    rdfs:isDefinedBy anzsic: ;
    skos:broader :J0000 ;
    skos:definition "An individual business entity whose predominant economic activity is Publishing (except Internet and Music Publishing)."@en ;
    skos:inScheme cs: ;
    skos:notation "J5400" ;
    skos:prefLabel "Publishing (except Internet and Music Publishing)"@en ;
    schema:temporalCoverage
        [
            schema:startTime "2026-02-10"^^xsd:date ;
        ] ;
.

:J5500
    a skos:Concept ;
    rdfs:isDefinedBy anzsic: ;
    skos:broader :J0000 ;
    skos:definition "An individual business entity whose predominant economic activity is Motion Picture and Sound Recording Activities."@en ;
    skos:inScheme cs: ;
    skos:notation "J5500" ;
    skos:prefLabel "Motion Picture and Sound Recording Activities"@en ;
    schema:temporalCoverage
        [
            schema:startTime "2026-02-10"^^xsd:date ;
        ] ;
.

:J5600
    a skos:Concept ;
    rdfs:isDefinedBy anzsic: ;
    skos:broader :J0000 ;
    skos:definition "An individual business entity whose predominant economic activity is Broadcasting (except Internet)."@en ;
    skos:inScheme cs: ;
    skos:notation "J5600" ;
    skos:prefLabel "Broadcasting (except Internet)"@en ;
    schema:temporalCoverage
        [
            schema:startTime "2026-02-10"^^xsd:date ;
        ] ;
.

:J5900
    a skos:Concept ;
    rdfs:isDefinedBy anzsic: ;
    skos:broader :J0000 ;
    skos:definition "An individual business entity whose predominant economic activity is Internet Service Providers, Web Search Portals and Data Processing Services."@en ;
    skos:inScheme cs: ;
    skos:notation "J5900" ;
    skos:prefLabel "Internet Service Providers, Web Search Portals and Data Processing Services"@en ;
    schema:temporalCoverage
        [
            schema:startTime "2026-02-10"^^xsd:date ;
        ] ;
.

:J6000
    a skos:Concept ;
    rdfs:isDefinedBy anzsic: ;
    skos:broader :J0000 ;
    skos:definition "An individual business entity whose predominant economic activity is Library and Other Information Services."@en ;
    skos:inScheme cs: ;
    skos:notation "J6000" ;
    skos:prefLabel "Library and Other Information Services"@en ;
    schema:temporalCoverage
        [
            schema:startTime "2026-02-10"^^xsd:date ;
        ] ;
.

:K6400
    a skos:Concept ;
    rdfs:isDefinedBy anzsic: ;
    skos:broader :K0000 ;
    skos:definition "An individual business entity whose predominant economic activity is Auxiliary Finance and Insurance Services."@en ;
    skos:inScheme cs: ;
    skos:notation "K6400" ;
    skos:prefLabel "Auxiliary Finance and Insurance Services"@en ;
    schema:temporalCoverage
        [
            schema:startTime "2026-02-10"^^xsd:date ;
        ] ;
.

:L6700
    a skos:Concept ;
    rdfs:isDefinedBy anzsic: ;
    skos:broader :L0000 ;
    skos:definition "An individual business entity whose predominant economic activity is Property Operators and Real Estate Services."@en ;
    skos:inScheme cs: ;
    skos:notation "L6700" ;
    skos:prefLabel "Property Operators and Real Estate Services"@en ;
    schema:temporalCoverage
        [
            schema:startTime "2026-02-10"^^xsd:date ;
        ] ;
.

:N7300
    a skos:Concept ;
    rdfs:isDefinedBy anzsic: ;
    skos:broader :N0000 ;
    skos:definition "An individual business entity whose predominant economic activity is Building Cleaning, Pest Control and Other Support Services."@en ;
    skos:inScheme cs: ;
    skos:notation "N7300" ;
    skos:prefLabel "Building Cleaning, Pest Control and Other Support Services"@en ;
    schema:temporalCoverage
        [
            schema:startTime "2026-02-10"^^xsd:date ;
        ] ;
.

:O7700
    a skos:Concept ;
    rdfs:isDefinedBy anzsic: ;
    skos:broader :O0000 ;
    skos:definition "An individual business entity whose predominant economic activity is Public Order, Safety and Regulatory Services."@en ;
    skos:inScheme cs: ;
    skos:notation "O7700" ;
    skos:prefLabel "Public Order, Safety and Regulatory Services"@en ;
    schema:temporalCoverage
        [
            schema:startTime "2026-02-10"^^xsd:date ;
        ] ;
.

:P8000
    a skos:Concept ;
    rdfs:isDefinedBy anzsic: ;
    skos:broader :P0000 ;
    skos:definition "An individual business entity whose predominant economic activity is Preschool and School Education."@en ;
    skos:inScheme cs: ;
    skos:notation "P8000" ;
    skos:prefLabel "Preschool and School Education"@en ;
    schema:temporalCoverage
        [
            schema:startTime "2026-02-10"^^xsd:date ;
        ] ;
.

:Q8700
    a skos:Concept ;
    rdfs:isDefinedBy anzsic: ;
    skos:broader :Q0000 ;
    skos:definition "An individual business entity whose predominant economic activity is Social Assistance Services."@en ;
    skos:inScheme cs: ;
    skos:notation "Q8700" ;
    skos:prefLabel "Social Assistance Services"@en ;
    schema:temporalCoverage
        [
            schema:startTime "2026-02-10"^^xsd:date ;
        ] ;
.

:R8900
    a skos:Concept ;
    rdfs:isDefinedBy anzsic: ;
    skos:broader :R0000 ;
    skos:definition "An individual business entity whose predominant economic activity is Heritage Activities."@en ;
    skos:inScheme cs: ;
    skos:notation "R8900" ;
    skos:prefLabel "Heritage Activities"@en ;
    schema:temporalCoverage
        [
            schema:startTime "2026-02-10"^^xsd:date ;
        ] ;
.

:F3300
    a skos:Concept ;
    rdfs:isDefinedBy anzsic: ;
    skos:broader :F0000 ;
    skos:definition "An individual business entity whose predominant economic activity is Basic Material Wholesaling."@en ;
    skos:inScheme cs: ;
    skos:notation "F3300" ;
    skos:prefLabel "Basic Material Wholesaling"@en ;
    schema:temporalCoverage
        [
            schema:startTime "2026-02-10"^^xsd:date ;
        ] ;
.

:F3700
    a skos:Concept ;
    rdfs:isDefinedBy anzsic: ;
    skos:broader :F0000 ;
    skos:definition "An individual business entity whose predominant economic activity is Other Goods Wholesaling."@en ;
    skos:inScheme cs: ;
    skos:notation "F3700" ;
    skos:prefLabel "Other Goods Wholesaling"@en ;
    schema:temporalCoverage
        [
            schema:startTime "2026-02-10"^^xsd:date ;
        ] ;
.

:H0000
    a skos:Concept ;
    rdfs:isDefinedBy anzsic: ;
    skos:definition "An individual business entity whose predominant economic activity is Accommodation and Food Services."@en ;
    skos:inScheme cs: ;
    skos:notation "H0000" ;
    skos:prefLabel "Accommodation and Food Services"@en ;
    skos:topConceptOf cs: ;
    schema:temporalCoverage
        [
            schema:startTime "2026-02-10"^^xsd:date ;
        ] ;
.

:H4500
    a skos:Concept ;
    rdfs:isDefinedBy anzsic: ;
    skos:broader :H0000 ;
    skos:definition "An individual business entity whose predominant economic activity is Food and Beverage Services."@en ;
    skos:inScheme cs: ;
    skos:notation "H4500" ;
    skos:prefLabel "Food and Beverage Services"@en ;
    schema:temporalCoverage
        [
            schema:startTime "2026-02-10"^^xsd:date ;
        ] ;
.

:I5200
    a skos:Concept ;
    rdfs:isDefinedBy anzsic: ;
    skos:broader :I0000 ;
    skos:definition "An individual business entity whose predominant economic activity is Transport Support Services."@en ;
    skos:inScheme cs: ;
    skos:notation "I5200" ;
    skos:prefLabel "Transport Support Services"@en ;
    schema:temporalCoverage
        [
            schema:startTime "2026-02-10"^^xsd:date ;
        ] ;
.

:K6300
    a skos:Concept ;
    rdfs:isDefinedBy anzsic: ;
    skos:broader :K0000 ;
    skos:definition "An individual business entity whose predominant economic activity is Insurance and Superannuation Funds."@en ;
    skos:inScheme cs: ;
    skos:notation "K6300" ;
    skos:prefLabel "Insurance and Superannuation Funds"@en ;
    schema:temporalCoverage
        [
            schema:startTime "2026-02-10"^^xsd:date ;
        ] ;
.

:L0000
    a skos:Concept ;
    rdfs:isDefinedBy anzsic: ;
    skos:definition "An individual business entity whose predominant economic activity is Rental, Hiring and Real Estate Services."@en ;
    skos:inScheme cs: ;
    skos:notation "L0000" ;
    skos:prefLabel "Rental, Hiring and Real Estate Services"@en ;
    skos:topConceptOf cs: ;
    schema:temporalCoverage
        [
            schema:startTime "2026-02-10"^^xsd:date ;
        ] ;
.

:M0000
    a skos:Concept ;
    rdfs:isDefinedBy anzsic: ;
    skos:definition "An individual business entity whose predominant economic activity is Professional, Scientific and Technical Services."@en ;
    skos:inScheme cs: ;
    skos:notation "M0000" ;
    skos:prefLabel "Professional, Scientific and Technical Services"@en ;
    skos:topConceptOf cs: ;
    schema:temporalCoverage
        [
            schema:startTime "2026-02-10"^^xsd:date ;
        ] ;
.

:N0000
    a skos:Concept ;
    rdfs:isDefinedBy anzsic: ;
    skos:definition "An individual business entity whose predominant economic activity is Administrative and Support Services."@en ;
    skos:inScheme cs: ;
    skos:notation "N0000" ;
    skos:prefLabel "Administrative and Support Services"@en ;
    skos:topConceptOf cs: ;
    schema:temporalCoverage
        [
            schema:startTime "2026-02-10"^^xsd:date ;
        ] ;
.

:N7200
    a skos:Concept ;
    rdfs:isDefinedBy anzsic: ;
    skos:broader :N0000 ;
    skos:definition "An individual business entity whose predominant economic activity is Administrative Services."@en ;
    skos:inScheme cs: ;
    skos:notation "N7200" ;
    skos:prefLabel "Administrative Services"@en ;
    schema:temporalCoverage
        [
            schema:startTime "2026-02-10"^^xsd:date ;
        ] ;
.

:R9100
    a skos:Concept ;
    rdfs:isDefinedBy anzsic: ;
    skos:broader :R0000 ;
    skos:definition "An individual business entity whose predominant economic activity is Sports and Recreation Activities."@en ;
    skos:inScheme cs: ;
    skos:notation "R9100" ;
    skos:prefLabel "Sports and Recreation Activities"@en ;
    schema:temporalCoverage
        [
            schema:startTime "2026-02-10"^^xsd:date ;
        ] ;
.

:S9400
    a skos:Concept ;
    rdfs:isDefinedBy anzsic: ;
    skos:broader :S0000 ;
    skos:definition "An individual business entity whose predominant economic activity is Repair and Maintenance."@en ;
    skos:inScheme cs: ;
    skos:notation "S9400" ;
    skos:prefLabel "Repair and Maintenance"@en ;
    schema:temporalCoverage
        [
            schema:startTime "2026-02-10"^^xsd:date ;
        ] ;
.

:X0000
    a skos:Concept ;
    rdfs:isDefinedBy anzsic: ;
    skos:definition "An individual business entity whose predominant economic activity is Undefined Industry."@en ;
    skos:inScheme cs: ;
    skos:notation "X0000" ;
    skos:prefLabel "Undefined Industry"@en ;
    skos:topConceptOf cs: ;
    schema:temporalCoverage
        [
            schema:startTime "2026-02-10"^^xsd:date ;
        ] ;
.

:C2000
    a skos:Concept ;
    rdfs:isDefinedBy anzsic: ;
    skos:broader :C0000 ;
    skos:definition "An individual business entity whose predominant economic activity is Non-Metallic Mineral Product Manufacturing."@en ;
    skos:inScheme cs: ;
    skos:notation "C2000" ;
    skos:prefLabel "Non-Metallic Mineral Product Manufacturing"@en ;
    schema:temporalCoverage
        [
            schema:startTime "2026-02-10"^^xsd:date ;
        ] ;
.

:C2100
    a skos:Concept ;
    rdfs:isDefinedBy anzsic: ;
    skos:altLabel "Metal Processing"@en ;
    skos:broader :C0000 ;
    skos:definition "An individual business entity whose predominant economic activity is Primary Metal and Metal Product Manufacturing."@en ;
    skos:inScheme cs: ;
    skos:notation "C2100" ;
    skos:prefLabel "Primary Metal and Metal Product Manufacturing"@en ;
    schema:temporalCoverage
        [
            schema:startTime "2026-02-10"^^xsd:date ;
        ] ;
.

:D2600
    a skos:Concept ;
    rdfs:isDefinedBy anzsic: ;
    skos:broader :D0000 ;
    skos:definition "An individual business entity whose predominant economic activity is Electricity Supply."@en ;
    skos:inScheme cs: ;
    skos:notation "D2600" ;
    skos:prefLabel "Electricity Supply"@en ;
    schema:temporalCoverage
        [
            schema:startTime "2026-02-10"^^xsd:date ;
        ] ;
.

:E0000
    a skos:Concept ;
    rdfs:isDefinedBy anzsic: ;
    skos:definition "An individual business entity whose predominant economic activity is Construction."@en ;
    skos:inScheme cs: ;
    skos:notation "E0000" ;
    skos:prefLabel "Construction"@en ;
    skos:topConceptOf cs: ;
    schema:temporalCoverage
        [
            schema:startTime "2026-02-10"^^xsd:date ;
        ] ;
.

:K0000
    a skos:Concept ;
    rdfs:isDefinedBy anzsic: ;
    skos:definition "An individual business entity whose predominant economic activity is Financial and Insurance Services."@en ;
    skos:inScheme cs: ;
    skos:notation "K0000" ;
    skos:prefLabel "Financial and Insurance Services"@en ;
    skos:topConceptOf cs: ;
    schema:temporalCoverage
        [
            schema:startTime "2026-02-10"^^xsd:date ;
        ] ;
.

:K6200
    a skos:Concept ;
    rdfs:isDefinedBy anzsic: ;
    skos:broader :K0000 ;
    skos:definition "An individual business entity whose predominant economic activity is Finance."@en ;
    skos:inScheme cs: ;
    skos:notation "K6200" ;
    skos:prefLabel "Finance"@en ;
    schema:temporalCoverage
        [
            schema:startTime "2026-02-10"^^xsd:date ;
        ] ;
.

:L6600
    a skos:Concept ;
    rdfs:isDefinedBy anzsic: ;
    skos:broader :L0000 ;
    skos:definition "An individual business entity whose predominant economic activity is Rental and Hiring Services (except Real Estate)."@en ;
    skos:inScheme cs: ;
    skos:notation "L6600" ;
    skos:prefLabel "Rental and Hiring Services (except Real Estate)"@en ;
    schema:temporalCoverage
        [
            schema:startTime "2026-02-10"^^xsd:date ;
        ] ;
.

:O0000
    a skos:Concept ;
    rdfs:isDefinedBy anzsic: ;
    skos:definition "An individual business entity whose predominant economic activity is Public Administration and Safety."@en ;
    skos:inScheme cs: ;
    skos:notation "O0000" ;
    skos:prefLabel "Public Administration and Safety"@en ;
    skos:topConceptOf cs: ;
    schema:temporalCoverage
        [
            schema:startTime "2026-02-10"^^xsd:date ;
        ] ;
.

:P0000
    a skos:Concept ;
    rdfs:isDefinedBy anzsic: ;
    skos:definition "An individual business entity whose predominant economic activity is Education and Training."@en ;
    skos:inScheme cs: ;
    skos:notation "P0000" ;
    skos:prefLabel "Education and Training"@en ;
    skos:topConceptOf cs: ;
    schema:temporalCoverage
        [
            schema:startTime "2026-02-10"^^xsd:date ;
        ] ;
.

:Q8500
    a skos:Concept ;
    rdfs:isDefinedBy anzsic: ;
    skos:broader :Q0000 ;
    skos:definition "An individual business entity whose predominant economic activity is Medical and Other Health Care Services."@en ;
    skos:inScheme cs: ;
    skos:notation "Q8500" ;
    skos:prefLabel "Medical and Other Health Care Services"@en ;
    schema:temporalCoverage
        [
            schema:startTime "2026-02-10"^^xsd:date ;
        ] ;
.

:S0000
    a skos:Concept ;
    rdfs:isDefinedBy anzsic: ;
    skos:definition "An individual business entity whose predominant economic activity is Other Services."@en ;
    skos:inScheme cs: ;
    skos:notation "S0000" ;
    skos:prefLabel "Other Services"@en ;
    skos:topConceptOf cs: ;
    schema:temporalCoverage
        [
            schema:startTime "2026-02-10"^^xsd:date ;
        ] ;
.

:C1300
    a skos:Concept ;
    rdfs:isDefinedBy anzsic: ;
    skos:broader :C0000 ;
    skos:definition "An individual business entity whose predominant economic activity is Textile, Leather, Clothing and Footwear Manufacturing."@en ;
    skos:inScheme cs: ;
    skos:notation "C1300" ;
    skos:prefLabel "Textile, Leather, Clothing and Footwear Manufacturing"@en ;
    schema:temporalCoverage
        [
            schema:startTime "2026-02-10"^^xsd:date ;
        ] ;
.

:C2200
    a skos:Concept ;
    rdfs:isDefinedBy anzsic: ;
    skos:broader :C0000 ;
    skos:definition "An individual business entity whose predominant economic activity is Fabricated Metal Product Manufacturing."@en ;
    skos:inScheme cs: ;
    skos:notation "C2200" ;
    skos:prefLabel "Fabricated Metal Product Manufacturing"@en ;
    schema:temporalCoverage
        [
            schema:startTime "2026-02-10"^^xsd:date ;
        ] ;
.

:D0000
    a skos:Concept ;
    rdfs:isDefinedBy anzsic: ;
    skos:definition "An individual business entity whose predominant economic activity is Electricity, Gas, Water and Waste Services."@en ;
    skos:inScheme cs: ;
    skos:notation "D0000" ;
    skos:prefLabel "Electricity, Gas, Water and Waste Services"@en ;
    skos:topConceptOf cs: ;
    schema:temporalCoverage
        [
            schema:startTime "2026-02-10"^^xsd:date ;
        ] ;
.

:E3200
    a skos:Concept ;
    rdfs:isDefinedBy anzsic: ;
    skos:broader :E0000 ;
    skos:definition "An individual business entity whose predominant economic activity is Construction Services."@en ;
    skos:inScheme cs: ;
    skos:notation "E3200" ;
    skos:prefLabel "Construction Services"@en ;
    schema:temporalCoverage
        [
            schema:startTime "2026-02-10"^^xsd:date ;
        ] ;
.

:O7500
    a skos:Concept ;
    rdfs:isDefinedBy anzsic: ;
    skos:broader :O0000 ;
    skos:definition "An individual business entity whose predominant economic activity is Public Administration."@en ;
    skos:inScheme cs: ;
    skos:notation "O7500" ;
    skos:prefLabel "Public Administration"@en ;
    schema:temporalCoverage
        [
            schema:startTime "2026-02-10"^^xsd:date ;
        ] ;
.

:Q0000
    a skos:Concept ;
    rdfs:isDefinedBy anzsic: ;
    skos:definition "An individual business entity whose predominant economic activity is Health Care and Social Assistance."@en ;
    skos:inScheme cs: ;
    skos:notation "Q0000" ;
    skos:prefLabel "Health Care and Social Assistance"@en ;
    skos:topConceptOf cs: ;
    schema:temporalCoverage
        [
            schema:startTime "2026-02-10"^^xsd:date ;
        ] ;
.

:R0000
    a skos:Concept ;
    rdfs:isDefinedBy anzsic: ;
    skos:definition "An individual business entity whose predominant economic activity is Arts and Recreation Services."@en ;
    skos:inScheme cs: ;
    skos:notation "R0000" ;
    skos:prefLabel "Arts and Recreation Services"@en ;
    skos:topConceptOf cs: ;
    schema:temporalCoverage
        [
            schema:startTime "2026-02-10"^^xsd:date ;
        ] ;
.

:S9500
    a skos:Concept ;
    rdfs:isDefinedBy anzsic: ;
    skos:broader :S0000 ;
    skos:definition "An individual business entity whose predominant economic activity is Personal and Other Services."@en ;
    skos:inScheme cs: ;
    skos:notation "S9500" ;
    skos:prefLabel "Personal and Other Services"@en ;
    schema:temporalCoverage
        [
            schema:startTime "2026-02-10"^^xsd:date ;
        ] ;
.

:A0000
    a skos:Concept ;
    rdfs:isDefinedBy anzsic: ;
    skos:definition "An individual business entity whose predominant economic activity is Agriculture, Forestry and Fishing."@en ;
    skos:inScheme cs: ;
    skos:notation "A0000" ;
    skos:prefLabel "Agriculture, Forestry and Fishing"@en ;
    skos:topConceptOf cs: ;
    schema:temporalCoverage
        [
            schema:startTime "2026-02-10"^^xsd:date ;
        ] ;
.

:B0000
    a skos:Concept ;
    rdfs:isDefinedBy anzsic: ;
    skos:definition "An individual business entity whose predominant economic activity is Mining."@en ;
    skos:inScheme cs: ;
    skos:notation "B0000" ;
    skos:prefLabel "Mining"@en ;
    skos:topConceptOf cs: ;
    schema:temporalCoverage
        [
            schema:startTime "2026-02-10"^^xsd:date ;
        ] ;
.

:C1800
    a skos:Concept ;
    rdfs:isDefinedBy anzsic: ;
    skos:broader :C0000 ;
    skos:definition "An individual business entity whose predominant economic activity is Basic Chemical and Chemical Product Manufacturing."@en ;
    skos:inScheme cs: ;
    skos:notation "C1800" ;
    skos:prefLabel "Basic Chemical and Chemical Product Manufacturing"@en ;
    schema:temporalCoverage
        [
            schema:startTime "2026-02-10"^^xsd:date ;
        ] ;
.

:G0000
    a skos:Concept ;
    rdfs:isDefinedBy anzsic: ;
    skos:definition "An individual business entity whose predominant economic activity is Retail Trade."@en ;
    skos:inScheme cs: ;
    skos:notation "G0000" ;
    skos:prefLabel "Retail Trade"@en ;
    skos:topConceptOf cs: ;
    schema:temporalCoverage
        [
            schema:startTime "2026-02-10"^^xsd:date ;
        ] ;
.

:C2400
    a skos:Concept ;
    rdfs:isDefinedBy anzsic: ;
    skos:broader :C0000 ;
    skos:definition "An individual business entity whose predominant economic activity is Machinery and Equipment Manufacturing."@en ;
    skos:inScheme cs: ;
    skos:notation "C2400" ;
    skos:prefLabel "Machinery and Equipment Manufacturing"@en ;
    schema:temporalCoverage
        [
            schema:startTime "2026-02-10"^^xsd:date ;
        ] ;
.

:F0000
    a skos:Concept ;
    rdfs:isDefinedBy anzsic: ;
    skos:definition "An individual business entity whose predominant economic activity is Wholesale Trade."@en ;
    skos:inScheme cs: ;
    skos:notation "F0000" ;
    skos:prefLabel "Wholesale Trade"@en ;
    skos:topConceptOf cs: ;
    schema:temporalCoverage
        [
            schema:startTime "2026-02-10"^^xsd:date ;
        ] ;
.

:G4200
    a skos:Concept ;
    rdfs:isDefinedBy anzsic: ;
    skos:broader :G0000 ;
    skos:definition "An individual business entity whose predominant economic activity is Other Store-Based Retailing."@en ;
    skos:inScheme cs: ;
    skos:notation "G4200" ;
    skos:prefLabel "Other Store-Based Retailing"@en ;
    schema:temporalCoverage
        [
            schema:startTime "2026-02-10"^^xsd:date ;
        ] ;
.

:J0000
    a skos:Concept ;
    rdfs:isDefinedBy anzsic: ;
    skos:definition "An individual business entity whose predominant economic activity is Information Media and Telecommunications."@en ;
    skos:inScheme cs: ;
    skos:notation "J0000" ;
    skos:prefLabel "Information Media and Telecommunications"@en ;
    skos:topConceptOf cs: ;
    schema:temporalCoverage
        [
            schema:startTime "2026-02-10"^^xsd:date ;
        ] ;
.

:M6900
    a skos:Concept ;
    rdfs:isDefinedBy anzsic: ;
    skos:broader :M0000 ;
    skos:definition "An individual business entity whose predominant economic activity is Professional, Scientific and Technical Services (Except Computer System Design and Related Services)."@en ;
    skos:inScheme cs: ;
    skos:notation "M6900" ;
    skos:prefLabel "Professional, Scientific and Technical Services (Except Computer System Design and Related Services)"@en ;
    schema:temporalCoverage
        [
            schema:startTime "2026-02-10"^^xsd:date ;
        ] ;
.

:A0100
    a skos:Concept ;
    rdfs:isDefinedBy anzsic: ;
    skos:broader :A0000 ;
    skos:definition "An individual business entity whose predominant economic activity is Agriculture."@en ;
    skos:inScheme cs: ;
    skos:notation "A0100" ;
    skos:prefLabel "Agriculture"@en ;
    schema:temporalCoverage
        [
            schema:startTime "2026-02-10"^^xsd:date ;
        ] ;
.

:C1100
    a skos:Concept ;
    rdfs:isDefinedBy anzsic: ;
    skos:broader :C0000 ;
    skos:definition "An individual business entity whose predominant economic activity is Food Product Manufacturing."@en ;
    skos:inScheme cs: ;
    skos:notation "C1100" ;
    skos:prefLabel "Food Product Manufacturing"@en ;
    schema:temporalCoverage
        [
            schema:startTime "2026-02-10"^^xsd:date ;
        ] ;
.

:I0000
    a skos:Concept ;
    rdfs:isDefinedBy anzsic: ;
    skos:definition "An individual business entity whose predominant economic activity is Transport, Postal and Warehousing."@en ;
    skos:inScheme cs: ;
    skos:notation "I0000" ;
    skos:prefLabel "Transport, Postal and Warehousing"@en ;
    skos:topConceptOf cs: ;
    schema:temporalCoverage
        [
            schema:startTime "2026-02-10"^^xsd:date ;
        ] ;
.

:C0000
    a skos:Concept ;
    dcterms:isReplacedBy :C0000-2 ;
    rdfs:isDefinedBy anzsic: ;
    skos:altLabel "Other Processing"@en ;
    skos:definition "An individual business entity whose predominant economic activity is Manufacturing."@en ;
    skos:inScheme cs: ;
    skos:notation "C0000" ;
    skos:prefLabel "Manufacturing"@en ;
    skos:topConceptOf cs: ;
    schema:temporalCoverage
        [
            schema:endTime "2026-02-12"^^xsd:date ;
            schema:startTime "2026-02-10"^^xsd:date ;
        ] ;
.

cs:
    a skos:ConceptScheme ;
    skos:definition "Suncorp's extended version of the Australian and New Zealand Standard Industrial Classification 2006 - Codes and Titles" ;
    skos:hasTopConcept
        :A0000 ,
        :B0000 ,
        :C0000 ,
        :C0000-2 ,
        :D0000 ,
        :E0000 ,
        :F0000 ,
        :G0000 ,
        :H0000 ,
        :I0000 ,
        :J0000 ,
        :K0000 ,
        :L0000 ,
        :M0000 ,
        :N0000 ,
        :O0000 ,
        :P0000 ,
        :Q0000 ,
        :R0000 ,
        :S0000 ,
        :X0000 ;
    skos:prefLabel "Suncorp's Extended ANZ Standard Industrial Classification 2006" ;
    schema:creator <https://linked.data.gov.au/org/abs> ;
    schema:dateCreated "2026-02-10"^^xsd:date ;
    schema:dateModified "2026-02-10"^^xsd:date ;
.
