@prefix skos: <http://www.w3.org/2004/02/skos/core#> .
@prefix dcterms: <http://purl.org/dc/terms/> .
@prefix xsd: <http://www.w3.org/2001/XMLSchema#> .
@prefix ex: <https://example.org/vocab/colors/> .

ex:scheme a skos:ConceptScheme ;
    skos:prefLabel "Example Colors"@en ;
    dcterms:description "A sample vocabulary demonstrating prez-lite. Replace with your own vocabularies."@en ;
    dcterms:created "2025-01-01"^^xsd:date ;
    dcterms:modified "2025-01-01"^^xsd:date ;
    skos:hasTopConcept ex:primary, ex:secondary .

ex:primary a skos:Concept ;
    skos:prefLabel "Primary Colors"@en ;
    skos:definition "Colors that cannot be created by mixing other colors."@en ;
    skos:inScheme ex:scheme ;
    skos:topConceptOf ex:scheme ;
    skos:narrower ex:red, ex:blue, ex:yellow .

ex:red a skos:Concept ;
    skos:prefLabel "Red"@en ;
    skos:notation "R" ;
    skos:definition "A primary color at the long wavelength end of the visible spectrum."@en ;
    skos:inScheme ex:scheme ;
    skos:broader ex:primary .

ex:blue a skos:Concept ;
    skos:prefLabel "Blue"@en ;
    skos:notation "B" ;
    skos:definition "A primary color between violet and green on the visible spectrum."@en ;
    skos:inScheme ex:scheme ;
    skos:broader ex:primary .

ex:yellow a skos:Concept ;
    skos:prefLabel "Yellow"@en ;
    skos:notation "Y" ;
    skos:definition "A primary color between orange and green on the visible spectrum."@en ;
    skos:inScheme ex:scheme ;
    skos:broader ex:primary .

ex:secondary a skos:Concept ;
    skos:prefLabel "Secondary Colors"@en ;
    skos:definition "Colors created by mixing two primary colors."@en ;
    skos:inScheme ex:scheme ;
    skos:topConceptOf ex:scheme ;
    skos:narrower ex:green, ex:orange, ex:purple .

ex:green a skos:Concept ;
    skos:prefLabel "Green"@en ;
    skos:notation "G" ;
    skos:definition "A secondary color created by mixing blue and yellow."@en ;
    skos:inScheme ex:scheme ;
    skos:broader ex:secondary .

ex:orange a skos:Concept ;
    skos:prefLabel "Orange"@en ;
    skos:notation "O" ;
    skos:definition "A secondary color created by mixing red and yellow."@en ;
    skos:inScheme ex:scheme ;
    skos:broader ex:secondary .

ex:purple a skos:Concept ;
    skos:prefLabel "Purple"@en ;
    skos:notation "P" ;
    skos:definition "A secondary color created by mixing red and blue."@en ;
    skos:inScheme ex:scheme ;
    skos:broader ex:secondary .
