PREFIX : <https://example.com/def/australian-states/>
PREFIX cs: <https://example.com/def/australian-states>
PREFIX owl: <http://www.w3.org/2002/07/owl#>
PREFIX rdfs: <http://www.w3.org/2000/01/rdf-schema#>
PREFIX schema: <https://schema.org/>
PREFIX skos: <http://www.w3.org/2004/02/skos/core#>
PREFIX xsd: <http://www.w3.org/2001/XMLSchema#>

cs:
    a
        owl:Ontology ,
        skos:ConceptScheme ;
    skos:prefLabel "Australian States and Territories" ;
    skos:definition "The states and territories of the Commonwealth of Australia, including their capital cities." ;
    schema:dateCreated "2026-01-01"^^xsd:date ;
    schema:dateModified "2026-02-19"^^xsd:date ;
    schema:creator <https://example.com/org/example> ;
    skos:hasTopConcept
        :states ,
        :territories ;
.

<https://example.com/org/example>
    a schema:Organization ;
    schema:name "Example Organisation" ;
    schema:url "https://example.com"^^xsd:anyURI ;
.

:states
    a skos:Concept ;
    rdfs:isDefinedBy cs: ;
    skos:definition "The six federated states of Australia." ;
    skos:inScheme cs: ;
    skos:prefLabel "States" ;
    skos:topConceptOf cs: ;
.

:nsw
    a skos:Concept ;
    rdfs:isDefinedBy cs: ;
    skos:broader :states ;
    skos:definition "The most populous state, located on the east coast. Capital: Sydney." ;
    skos:inScheme cs: ;
    skos:prefLabel "New South Wales" ;
    skos:altLabel "NSW" ;
    skos:notation "NSW"^^xsd:string ;
.

:vic
    a skos:Concept ;
    rdfs:isDefinedBy cs: ;
    skos:broader :states ;
    skos:definition "A southeastern state and the smallest on the mainland. Capital: Melbourne." ;
    skos:inScheme cs: ;
    skos:prefLabel "Victoria" ;
    skos:altLabel "VIC" ;
    skos:notation "VIC"^^xsd:string ;
.

:qld
    a skos:Concept ;
    rdfs:isDefinedBy cs: ;
    skos:broader :states ;
    skos:definition "The second-largest state, occupying the northeast. Capital: Brisbane." ;
    skos:inScheme cs: ;
    skos:prefLabel "Queensland" ;
    skos:altLabel "QLD" ;
    skos:notation "QLD"^^xsd:string ;
.

:wa
    a skos:Concept ;
    rdfs:isDefinedBy cs: ;
    skos:broader :states ;
    skos:definition "The largest state by area, covering the western third of the continent. Capital: Perth." ;
    skos:inScheme cs: ;
    skos:prefLabel "Western Australia" ;
    skos:altLabel "WA" ;
    skos:notation "WA"^^xsd:string ;
.

:sa
    a skos:Concept ;
    rdfs:isDefinedBy cs: ;
    skos:broader :states ;
    skos:definition "A southern state bordered by all other mainland states and the Northern Territory. Capital: Adelaide." ;
    skos:inScheme cs: ;
    skos:prefLabel "South Australia" ;
    skos:altLabel "SA" ;
    skos:notation "SA"^^xsd:string ;
.

:tas
    a skos:Concept ;
    rdfs:isDefinedBy cs: ;
    skos:broader :states ;
    skos:definition "An island state south of the mainland. Capital: Hobart." ;
    skos:inScheme cs: ;
    skos:prefLabel "Tasmania" ;
    skos:altLabel "TAS" ;
    skos:notation "TAS"^^xsd:string ;
.

:territories
    a skos:Concept ;
    rdfs:isDefinedBy cs: ;
    skos:definition "The major self-governing internal territories of Australia." ;
    skos:inScheme cs: ;
    skos:prefLabel "Territories" ;
    skos:topConceptOf cs: ;
.

:act
    a skos:Concept ;
    rdfs:isDefinedBy cs: ;
    skos:broader :territories ;
    skos:definition "An enclave within New South Wales containing the national capital, Canberra." ;
    skos:inScheme cs: ;
    skos:prefLabel "Australian Capital Territory" ;
    skos:altLabel "ACT" ;
    skos:notation "ACT"^^xsd:string ;
.

:nt
    a skos:Concept ;
    rdfs:isDefinedBy cs: ;
    skos:broader :territories ;
    skos:definition "A territory in the centre and central north of the continent. Capital: Darwin." ;
    skos:inScheme cs: ;
    skos:prefLabel "Northern Territory" ;
    skos:altLabel "NT" ;
    skos:notation "NT"^^xsd:string ;
.
